Refactored storage of key permissions, solving several problems. Everything but the protocol compilse now, but many goals remain to be filled in.

KeyManagement/RealWorld.v
@@ -35,10 +35,12 @@ Lemma key_eq_dec :
   decide equality; auto using Nat.eq_dec, key_usage_eq_dec, key_type_eq_dec.
 Defined.
 
-Record key_permission :=
-  MkKeyPerm { key_ref            : key_identifier
-            ; has_private_access : bool
-            }.
+Definition key_permission : Set := key_identifier * bool.
+
+(* Record key_permission := *)
+(*   MkKeyPerm { key_ref            : key_identifier *)
+(*             ; has_private_access : bool *)
+(*             }. *)
 
 Lemma key_permission_eq_dec :
   forall kp1 kp2 : key_permission, { kp1 = kp2 } + { kp1 <> kp2 }.
@@ -100,7 +102,7 @@ Definition cipher_signing_key (c : cipher) :=
 
 Definition queued_messages := list (sigT message).
 Definition keys            := NatMap.t key.
-Definition key_perms       := NatMap.t key_permission.
+Definition key_perms       := NatMap.t bool.
 Definition ciphers         := NatMap.t cipher.
 
 Inductive msg_accepted_by_pattern (cs : ciphers) (pat : msg_pat) : forall {t : type}, message t -> Prop :=
@@ -139,11 +141,18 @@ Ltac clean_map_lookups1 :=
   | [ H1 : ?m $? ?k = _ , H2 : ?m $? ?k = _ |- _] => rewrite H1 in H2
   end.
 
+(* Ltac contra_map_lookup := *)
+(*   match goal with *)
+(*   | [ H1 : ?ks $? ?k = Some _, H2 : ?ks $? ?k = None |- _ ] => rewrite H1 in H2; invert H2 *)
+(*   | [ H : ?v1 <> ?v2, H1 : ?ks $? ?k = Some ?v1, H2 : ?ks $? ?k = Some ?v2 |- _ ] => rewrite H1 in H2; invert H2; contradiction *)
+(*   end. *)
+
 Ltac contra_map_lookup :=
-  match goal with
-  | [ H1 : ?ks $? ?k = Some _, H2 : ?ks $? ?k = None |- _ ] => rewrite H1 in H2; invert H2
-  | [ H : ?v1 <> ?v2, H1 : ?ks $? ?k = Some ?v1, H2 : ?ks $? ?k = Some ?v2 |- _ ] => rewrite H1 in H2; invert H2; contradiction
-  end.
+  repeat
+    match goal with
+    | [ H1 : ?ks1 $? ?k = _, H2 : ?ks2 $? ?k = _ |- _ ] => rewrite H1 in H2; invert H2
+    | [ H : ?v1 <> ?v2, H1 : ?ks $? ?k = Some ?v1, H2 : ?ks $? ?k = Some ?v2 |- _ ] => rewrite H1 in H2; invert H2; contradiction
+    end; try discriminate.
 
 Ltac clean_map_lookups :=
   (repeat clean_map_lookups1);
@@ -160,6 +169,22 @@ Ltac split_ors :=
          | [ H : _ \/ _ |- _ ] => destruct H
          end.
 
+Ltac Equal_eq :=
+  repeat
+    match goal with
+    | [ H : Equal _ _ |- _] => apply map_eq_Equal in H; subst
+    end.
+
+Ltac context_map_rewrites :=
+  repeat
+    match goal with
+    | [ H : ?m $? ?k = _ |- context[?m $? ?k] ] => rewrite H
+    | [ H : match ?matchee with _ => _ end $? _ = _
+     ,  H1 : ?matchee = _ |- _] => rewrite H1 in H
+    | [ H : match ?matchee with _ => _ end = _
+     ,  H1 : ?matchee = _ |- _] => rewrite H1 in H
+    end.
+
 Hint Extern 1 (~ In _ _) => rewrite not_find_in_iff.
 
 Section SafeMessages.
@@ -167,10 +192,10 @@ Section SafeMessages.
   Variable honestk advk : key_perms.
 
   Definition has_private_key (k : key_permission) : bool :=
-    match (all_keys $? k.(key_ref)) with
+    match (all_keys $? fst k) with
     | None      => false
     | Some (MkCryptoKey _ _ SymKey)  => true
-    | Some (MkCryptoKey _ _ AsymKey) => k.(has_private_access)
+    | Some (MkCryptoKey _ _ AsymKey) => snd k
     end.
 
     Definition honest_key (k : key_identifier) : bool :=
@@ -183,8 +208,8 @@ Section SafeMessages.
       end
     | Some (MkCryptoKey _ _ AsymKey) =>
       match honestk $? k with
-      | None                        => false
-      | Some (MkKeyPerm _ has_priv) => has_priv
+      | None          => false
+      | Some has_priv => has_priv
       end
     end.
 
@@ -205,9 +230,9 @@ Section SafeMessages.
   Fixpoint msg_needs_encryption {t} (msg : message t) : bool :=
     match msg with
     | Plaintext _        => false
-    | KeyMessage k       => match all_keys $? k.(key_ref) with
+    | KeyMessage k       => match all_keys $? fst k with
                            | None   => false
-                           | Some _ => honest_key k.(key_ref)
+                           | Some _ => honest_key (fst k)
                            end
     | MsgPair msg1 msg2  => msg_needs_encryption msg1 || msg_needs_encryption msg2
     | SignedCiphertext _ => false
@@ -290,8 +315,6 @@ Record user_data (A : Type) :=
       key_heap : key_perms
     ; protocol : user_cmd A
     ; msg_heap : queued_messages
-      (* msg_heap : user_msg_heap ; *)
-      (* is_admin : bool *)
     }.
 
 Definition honest_users A := user_list (user_data A).
@@ -309,8 +332,7 @@ Definition is_powerless {B} (usr : user_data B) : bool :=
 && match usr.(msg_heap) with
    | [] => true
    | _  => false
-   end
-.
+   end.
 
 Record universe (A B : Type) :=
   mkUniverse {
@@ -320,181 +342,131 @@ Record universe (A B : Type) :=
     ; all_keys    : keys
     }.
 
-(* Definition canonical_key (k1 k2 : key) := *)
-(*   match Coq.Init.Nat.compare k1.(keyId) k2.(keyId) with *)
-(*   | Gt => k1 *)
-(*   | Lt => k2 *)
-(*   | Eq => *)
-(*     match (k1.(keyUsage), k2.(keyUsage)) with *)
-(*     | (Signing, Encryption) => k1 *)
-(*     | (Encryption, Signing) => k2 *)
-(*     | _                     => *)
-(*       match (k1.(keyType), k2.(keyType)) with *)
-(*       | (SymKey, _) => k1 *)
-(*       | (_, SymKey) => k2 *)
-(*       | (AsymKey b1, AsymKey b2) => if b1 then k1 else k2 *)
-(*       end *)
-(*     end *)
-(*   end. *)
-
 Definition keys_good (ks : keys) : Prop :=
   forall k_id k,
     ks $? k_id = Some k
     -> keyId k = k_id.
 
-Definition key_perms_good (perms : key_perms) : Prop :=
-  forall k_id k,
-      perms $? k_id = Some k
-    -> key_ref k = k_id.
+Definition greatest_permission (kp1 kp2 : bool) : bool :=
+  kp1 || kp2.
 
-Section KeyPermissions.
-  Variable perms : key_perms.
-  Variable gperms : key_perms_good perms.
-
-  (* Definition greatest_permission (kp1 kp2 : key_permission) (eq_proof : kp1.(key_ref) = kp2.(key_ref)) : key_permission := *)
-  (*   match (kp1,kp2) with *)
-  (*   | (MkKeyPerm _ has_priv1, MkKeyPerm _ has_priv2) => MkKeyPerm kp1.(key_ref) (has_priv1 || has_priv2) *)
-  (*   end. *)
-
-  Definition greatest_permission (kp1 kp2 : key_permission) : key_permission :=
-    match (kp1,kp2) with
-    | (MkKeyPerm _ has_priv1, MkKeyPerm _ has_priv2) => MkKeyPerm kp1.(key_ref) (has_priv1 || has_priv2)
+Definition add_key_perm (k : key_identifier)(kp : bool) (perms : key_perms) : key_perms :=
+    match perms $? k with
+    | None     => perms $+ (k, kp)
+    | Some kp' => perms $+ (k, greatest_permission kp kp')
     end.
-
-  Definition add_key_perm (kp : key_permission) : key_perms :=
-    match perms $? key_ref kp with
-    | None     => perms $+ (key_ref kp, kp)
-    | Some kp' => perms $+ (key_ref kp, greatest_permission kp kp')
-    end.
-
-  Lemma add_key_keeps_good :
-    forall kp perms',
-      perms' = add_key_perm kp
-      -> key_perms_good perms'.
-  Proof.
-    intros.
-    unfold key_perms_good in *; intros.
-    unfold add_key_perm in *.
-    destruct kp; subst; simpl in *.
-    cases (k_id ==n key_ref0); cases (perms $? key_ref0); subst; clean_map_lookups; auto.
-    unfold greatest_permission; destruct k0; simpl; trivial.
-  Qed.
-
-End KeyPermissions.
 
 Lemma greatest_permission_refl :
   forall k,
     greatest_permission k k = k.
 Proof.
-  unfold greatest_permission; intros; destruct k; simpl in *; rewrite orb_diag; trivial.
+  unfold greatest_permission; auto using orb_diag.
 Qed.
 
 Lemma greatest_permission_symm :
-  forall k1 k2,
-    key_ref k1 = key_ref k2
-    -> greatest_permission k1 k2 = greatest_permission k2 k1.
+  forall kp1 kp2,
+    greatest_permission kp1 kp2 = greatest_permission kp2 kp1.
 Proof.
-  unfold greatest_permission; intros; destruct k1; destruct k2; simpl in *; subst; rewrite orb_comm; trivial.
+  unfold greatest_permission; auto using orb_comm.
 Qed.
 
-Definition add_key_perm_fold_fn (_ : key_identifier) (kp : key_permission) (perms : key_perms) : key_perms :=
-  add_key_perm perms kp.
-
 Definition merge_perms (ks ks' : key_perms) : key_perms :=
-  fold add_key_perm_fold_fn ks ks'.
+  fold add_key_perm ks ks'.
 
 Notation "m1 $k++ m2" := (merge_perms m2 m1) (at level 50, left associativity).
 
-Lemma add_key_perm_fold_fn_proper :
-  Proper (eq  ==>  eq  ==>  eq  ==>  eq ) add_key_perm_fold_fn.
+Lemma add_key_perm_proper :
+  Proper (eq  ==>  eq  ==>  eq  ==>  eq ) add_key_perm.
 Proof.
   unfold Proper, respectful; intros; subst; trivial.
 Qed.
 
-Lemma add_key_perm_fold_fn_proper_Equal :
-  Proper (eq  ==>  eq  ==>  Equal  ==>  Equal ) add_key_perm_fold_fn.
+Lemma add_key_perm_proper_Equal :
+  Proper (eq  ==>  eq  ==>  Equal  ==>  Equal ) add_key_perm.
 Proof.
-  unfold Proper, respectful; intros.
-  apply map_eq_Equal in H1; subst; unfold Equal; intros; trivial.
+  unfold Proper, respectful; intros; Equal_eq;
+    unfold Equal; intros; trivial.
 Qed.
 
-Lemma add_key_perm_fold_fn_transpose' :
-  forall (k k' : nat) (e e' : key_permission) a,
-    k <> k'
-    -> Equal
-        match match a $? key_ref e' with
-              | Some kp' => a $+ (key_ref e', greatest_permission e' kp')
-              | None => a $+ (key_ref e', e')
-              end $? key_ref e with
-        | Some kp' =>
-          match a $? key_ref e' with
-          | Some kp'0 => a $+ (key_ref e', greatest_permission e' kp'0)
-          | None => a $+ (key_ref e', e')
-          end $+ (key_ref e, greatest_permission e kp')
-        | None => match a $? key_ref e' with
-                 | Some kp' => a $+ (key_ref e', greatest_permission e' kp')
-                 | None => a $+ (key_ref e', e')
-                 end $+ (key_ref e, e)
-        end
-        match match a $? key_ref e with
-              | Some kp' => a $+ (key_ref e, greatest_permission e kp')
-              | None => a $+ (key_ref e, e)
-              end $? key_ref e' with
-        | Some kp' =>
-          match a $? key_ref e with
-          | Some kp'0 => a $+ (key_ref e, greatest_permission e kp'0)
-          | None => a $+ (key_ref e, e)
-          end $+ (key_ref e', greatest_permission e' kp')
-        | None => match a $? key_ref e with
-                 | Some kp' => a $+ (key_ref e, greatest_permission e kp')
-                 | None => a $+ (key_ref e, e)
-                 end $+ (key_ref e', e')
-        end.
+(* Lemma add_key_perm_fold_fn_transpose' : *)
+(*   forall (k k' : nat) (e e' : key_permission) a, *)
+(*     k <> k' *)
+(*     -> Equal *)
+(*         match match a $? key_ref e' with *)
+(*               | Some kp' => a $+ (key_ref e', greatest_permission e' kp') *)
+(*               | None => a $+ (key_ref e', e') *)
+(*               end $? key_ref e with *)
+(*         | Some kp' => *)
+(*           match a $? key_ref e' with *)
+(*           | Some kp'0 => a $+ (key_ref e', greatest_permission e' kp'0) *)
+(*           | None => a $+ (key_ref e', e') *)
+(*           end $+ (key_ref e, greatest_permission e kp') *)
+(*         | None => match a $? key_ref e' with *)
+(*                  | Some kp' => a $+ (key_ref e', greatest_permission e' kp') *)
+(*                  | None => a $+ (key_ref e', e') *)
+(*                  end $+ (key_ref e, e) *)
+(*         end *)
+(*         match match a $? key_ref e with *)
+(*               | Some kp' => a $+ (key_ref e, greatest_permission e kp') *)
+(*               | None => a $+ (key_ref e, e) *)
+(*               end $? key_ref e' with *)
+(*         | Some kp' => *)
+(*           match a $? key_ref e with *)
+(*           | Some kp'0 => a $+ (key_ref e, greatest_permission e kp'0) *)
+(*           | None => a $+ (key_ref e, e) *)
+(*           end $+ (key_ref e', greatest_permission e' kp') *)
+(*         | None => match a $? key_ref e with *)
+(*                  | Some kp' => a $+ (key_ref e, greatest_permission e kp') *)
+(*                  | None => a $+ (key_ref e, e) *)
+(*                  end $+ (key_ref e', e') *)
+(*         end. *)
+(* Proof. *)
+(*   unfold Equal; intros. *)
+(*   destruct e; destruct e'; simpl. *)
+(*   cases (key_ref0 ==n key_ref1); subst; auto. *)
+(*   - cases (a $? key_ref1); clean_map_lookups; simpl. *)
+(*     + cases (y ==n key_ref1); subst; clean_map_lookups; auto. *)
+(*       unfold greatest_permission; destruct k0; simpl; auto. *)
+(*       rewrite !orb_assoc. *)
+(*       rewrite orb_comm with (b1:=has_private_access0). *)
+(*       trivial. *)
+(*     + unfold greatest_permission; simpl. *)
+(*       cases (y ==n key_ref1); subst; clean_map_lookups; auto. *)
+(*       rewrite orb_comm; trivial. *)
+(*   - cases (a $? key_ref0); cases (a $? key_ref1); clean_map_lookups; *)
+(*       rewrite Heq; rewrite Heq0; clean_map_lookups; *)
+(*         unfold greatest_permission; try destruct k0; try destruct k1; simpl; *)
+(*           cases (y ==n key_ref0); cases (y ==n key_ref1); subst; clean_map_lookups; try contradiction; auto. *)
+(* Qed. *)
+
+Lemma add_key_perm_transpose :
+  transpose_neqkey eq add_key_perm.
 Proof.
-  unfold Equal; intros.
-  destruct e; destruct e'; simpl.
-  cases (key_ref0 ==n key_ref1); subst; auto.
-  - cases (a $? key_ref1); clean_map_lookups; simpl.
-    + cases (y ==n key_ref1); subst; clean_map_lookups; auto.
-      unfold greatest_permission; destruct k0; simpl; auto.
-      rewrite !orb_assoc.
-      rewrite orb_comm with (b1:=has_private_access0).
-      trivial.
-    + unfold greatest_permission; simpl.
-      cases (y ==n key_ref1); subst; clean_map_lookups; auto.
-      rewrite orb_comm; trivial.
-  - cases (a $? key_ref0); cases (a $? key_ref1); clean_map_lookups;
-      rewrite Heq; rewrite Heq0; clean_map_lookups;
-        unfold greatest_permission; try destruct k0; try destruct k1; simpl;
-          cases (y ==n key_ref0); cases (y ==n key_ref1); subst; clean_map_lookups; try contradiction; auto.
+  unfold transpose_neqkey, add_key_perm; intros.
+  apply map_eq_Equal; unfold Equal; intros;
+    cases (a $? k); cases (a $? k');
+      repeat (context_map_rewrites; clean_map_lookups);
+      cases (y ==n k); cases (y ==n k'); subst; clean_map_lookups; trivial; contradiction.
 Qed.
 
-Lemma add_key_perm_fold_fn_transpose :
-  transpose_neqkey eq add_key_perm_fold_fn.
+Lemma add_key_perm_transpose_Equal :
+  transpose_neqkey Equal add_key_perm.
 Proof.
-  unfold transpose_neqkey, add_key_perm_fold_fn, add_key_perm; intros.
-  apply map_eq_Equal; eauto using add_key_perm_fold_fn_transpose'.
+  unfold transpose_neqkey, add_key_perm; intros.
+  unfold Equal; intros;
+    cases (a $? k); cases (a $? k');
+      repeat (context_map_rewrites; clean_map_lookups);
+      cases (y ==n k); cases (y ==n k'); subst; clean_map_lookups; trivial; contradiction.
 Qed.
 
-Lemma add_key_perm_fold_fn_transpose_Equal :
-  transpose_neqkey Equal add_key_perm_fold_fn.
-Proof.
-  unfold transpose_neqkey, add_key_perm_fold_fn, add_key_perm; intros.
-  eauto using add_key_perm_fold_fn_transpose'.
-Qed.
-
-Hint Resolve add_key_perm_fold_fn_proper add_key_perm_fold_fn_transpose
-     add_key_perm_fold_fn_proper_Equal add_key_perm_fold_fn_transpose_Equal.
-
-(* Definition merge_keys (ks ks' : keys) : keys := *)
-(*   fold add_key ks ks'. *)
-
-(* Notation "m1 $k++ m2" := (merge_keys m2 m1) (at level 50, left associativity). *)
+Hint Resolve
+     add_key_perm_proper       add_key_perm_transpose
+     add_key_perm_proper_Equal add_key_perm_transpose_Equal.
 
 Fixpoint findKeys {t} (msg : message t) : key_perms :=
   match msg with
   | Plaintext _        => $0
-  | KeyMessage k       => $0 $+ (key_ref k, k)
+  | KeyMessage k       => $0 $+ (fst k, snd k)
   | MsgPair msg1 msg2  => (findKeys msg1) $k++ (findKeys msg2)
   | SignedCiphertext _ => $0
   | Signature m _      => findKeys m
@@ -518,78 +490,53 @@ Definition adv_no_honest_keys (all_keys : keys) (honestk advk : key_perms) : Pro
       | None   => True
       | Some _ => False
       end
-    | Some (MkCryptoKey _ _ AsymKey) => 
+    | Some (MkCryptoKey _ _ AsymKey) =>
       match advk $? k_id with
-      | None                     => True
-      | Some (MkKeyPerm _ false) => True
-      | Some (MkKeyPerm _ true)  => honest_key all_keys honestk k_id = false
+      | None       => True
+      | Some false => True
+      | Some true  => honest_key all_keys honestk k_id = false
       end
     end.
+
+Definition universe_ok {A B} (U : universe A B) : Prop :=
+  let honestk := findUserKeys U.(users)
+  in  (forall u_id (u_d : user_data A), U.(users) $? u_id = Some u_d -> message_queue_safe U.(all_keys) honestk (u_d.(msg_heap)) = true)
+    /\ message_queue_safe U.(all_keys) honestk U.(adversary).(msg_heap) = true
+    /\ keys_good U.(all_keys)
+    /\ adv_no_honest_keys U.(all_keys) honestk U.(adversary).(key_heap).
 
 Section KeyMergeTheorems.
   Variable all_keys : keys.
   Variable honestk advk : key_perms.
-
   Variable k_good      : keys_good all_keys.
-  Variable honest_good : key_perms_good honestk.
-  Variable adv_good    : key_perms_good advk.
 
   Hint Resolve empty_Empty.
 
   Ltac progress_fold_add1 :=
     match goal with
-    | [ H : fold add_key_perm_fold_fn (_ $+ (_,_)) _ $? _ = _ |- _ ] => rewrite fold_add in H
+    | [ H : fold add_key_perm (_ $+ (_,_)) _ $? _ = _ |- _ ] => rewrite fold_add in H
     | [ H : _ $k++ (_ $+ (_,_)) $? _ = _ |- _ ] => unfold merge_perms in H; rewrite fold_add in H
-    | [ |- context[ fold add_key_perm_fold_fn (_ $+ (_,_)) _ ] ] => rewrite fold_add
+    | [ |- context[ fold add_key_perm (_ $+ (_,_)) _ ] ] => rewrite fold_add
     | [ |- context[ _ $k++ (_ $+ (_,_))] ] => unfold merge_perms; rewrite fold_add
     end.
 
   Lemma merge_perms_notation :
     forall ks1 ks2,
-      fold add_key_perm_fold_fn ks2 ks1 = ks1 $k++ ks2.
+      fold add_key_perm ks2 ks1 = ks1 $k++ ks2.
     unfold merge_perms; trivial.
   Qed.
 
-  Lemma key_perms_good_add :
-    forall ks k_id kp,
-      key_perms_good (ks $+ (k_id, kp))
-      -> ~ In k_id ks
-      -> key_ref kp = k_id
-      /\ key_perms_good ks.
-  Proof.
-    intros.
-    unfold key_perms_good in H.
-    split.
-    - apply H; clean_map_lookups; trivial.
-    - unfold key_perms_good; intros; cases (k_id ==n k_id0); subst; clean_map_lookups;
-        eapply H; clean_map_lookups; auto.
-  Qed.
-
-  Lemma empty_key_perms_good :
-    key_perms_good $0.
-  Proof.
-    unfold key_perms_good; intros; invert H.
-  Qed.
-
-  Hint Resolve empty_key_perms_good.
-
   Lemma merge_perms_left_identity :
     forall ks,
-        key_perms_good ks
-      -> $0 $k++ ks = ks.
+      $0 $k++ ks = ks.
   Proof.
-    induction ks using P.map_induction_bis; intros.
-    - apply map_eq_Equal in H; subst; auto.
-    - apply fold_Empty; eauto.
-    - unfold merge_perms.
-      rewrite fold_add; auto.
-      apply key_perms_good_add in H0; auto; split_ands.
+    induction ks using P.map_induction_bis; intros; Equal_eq; auto.
 
-      rewrite merge_perms_notation.
-      unfold add_key_perm_fold_fn, add_key_perm.
-      rewrite IHks; auto.
-
-      case_eq (ks $? key_ref e); intros; subst; clean_map_lookups; trivial.
+    progress_fold_add1; auto.
+    rewrite merge_perms_notation.
+    unfold add_key_perm; auto.
+    rewrite IHks; auto.
+    case_eq (ks $? x); intros; subst; clean_map_lookups; trivial.
   Qed.
 
   Lemma merge_keys_right_identity :
@@ -599,525 +546,356 @@ Section KeyMergeTheorems.
     unfold merge_perms; intros; rewrite fold_Empty; eauto.
   Qed.
 
-  Lemma key_perms_merge_still_good :
-    forall ks2 ks1,
-      key_perms_good ks1
-      -> key_perms_good ks2
-      -> key_perms_good (ks1 $k++ ks2).
-  Proof.
-    induction ks2 using P.map_induction_bis; intros.
-    - apply map_eq_Equal in H; subst; auto.
-    - rewrite merge_keys_right_identity; auto.
-    - apply key_perms_good_add in H1; split_ands; subst; auto.
-      progress_fold_add1; auto.
-      rewrite merge_perms_notation.
-      unfold add_key_perm_fold_fn, add_key_perm; simpl.
-      cases (ks1 $k++ ks2 $? key_ref e).
-      + unfold key_perms_good; intros.
-        specialize (IHks2 _ H0 H2).
-        assert (ks1 $k++ ks2 $? key_ref e = Some k) as EQ by assumption; apply IHks2 in EQ.
-        cases (key_ref e ==n k_id); subst; clean_map_lookups; auto.
-        unfold greatest_permission; destruct e; destruct k; auto.
-      + unfold key_perms_good; intros.
-        cases (key_ref e ==n k_id); subst; clean_map_lookups; auto.
-        specialize (IHks2 _ H0 H2); auto.
-  Qed.
+  Hint Rewrite merge_keys_right_identity merge_perms_left_identity.
 
   Lemma merge_perms_adds_no_new_perms :
     forall ks2 k ks1,
         ks1 $? k = None
       -> ks2 $? k = None
-      -> key_perms_good ks2
       -> (ks1 $k++ ks2) $? k = None.
   Proof.
-    induction ks2 using P.map_induction_bis; intros; auto.
-    - apply map_eq_Equal in H; subst; auto.
-    - progress_fold_add1; auto.
-      rewrite merge_perms_notation.
-      unfold add_key_perm_fold_fn, add_key_perm.
-      apply key_perms_good_add in H2; split_ands; subst; auto.
-      case (key_ref e ==n k); intros; subst; clean_map_lookups.
-      cases (ks1 $k++ ks2 $? key_ref e); clean_map_lookups; auto.
+    induction ks2 using P.map_induction_bis; intros; Equal_eq; auto.
+    progress_fold_add1; auto.
+    rewrite merge_perms_notation.
+    unfold add_key_perm.
+    case (x ==n k); intros; subst; clean_map_lookups.
+    cases (ks1 $k++ ks2 $? x); clean_map_lookups; auto.
   Qed.
+
+  Hint Resolve merge_perms_adds_no_new_perms.
 
   Lemma merge_perms_came_from_somewhere1 :
     forall ks2 ks1 k v,
         ks1 $k++ ks2 $? k = Some v
-      -> key_perms_good ks1
-      -> key_perms_good ks2
       -> ks2 $? k = None
       -> ks1 $? k = Some v.
   Proof.
-    induction ks2 using P.map_induction_bis; intros.
-
-    - apply map_eq_Equal in H; subst; eauto.
-    - rewrite merge_keys_right_identity in H; auto.
-    - case (x ==n k); intros; subst; clean_map_lookups.
-      apply key_perms_good_add in H2; split_ands; subst; auto.
-      progress_fold_add1; auto.
-      rewrite merge_perms_notation in H0.
-      unfold add_key_perm_fold_fn, add_key_perm in H0.
-      cases (ks1 $k++ ks2 $? key_ref e); clean_map_lookups; eauto.
+    induction ks2 using P.map_induction_bis; intros; Equal_eq; auto.
+    case (x ==n k); intros; subst; clean_map_lookups.
+    progress_fold_add1; auto.
+    rewrite merge_perms_notation in *.
+    unfold add_key_perm in *.
+    cases (ks1 $k++ ks2 $? x); clean_map_lookups; auto.
   Qed.
 
   Lemma merge_perms_came_from_somewhere2 :
     forall ks2 ks1 k v,
         ks1 $k++ ks2 $? k = Some v
-      -> key_perms_good ks1
-      -> key_perms_good ks2
       -> ks1 $? k = None
       -> ks2 $? k = Some v.
   Proof.
-    induction ks2 using P.map_induction_bis; intros.
-    - apply map_eq_Equal in H; subst; eauto.
+    induction ks2 using P.map_induction_bis; intros; Equal_eq; eauto.
     - rewrite merge_keys_right_identity in H; clean_map_lookups.
-    - apply key_perms_good_add in H2; split_ands; subst; auto.
-      case (k ==n key_ref e); intros; subst; clean_map_lookups.
-      + progress_fold_add1; auto.
-        rewrite merge_perms_notation in H0.
-        unfold add_key_perm_fold_fn, add_key_perm in H0.
-        assert (ks1 $k++ ks2 $? key_ref e = None) by eauto using merge_perms_adds_no_new_perms.
-        rewrite H2 in H0; clean_map_lookups; trivial.
-      + progress_fold_add1; auto.
-        rewrite merge_perms_notation in H0.
-        unfold add_key_perm_fold_fn, add_key_perm in H0.
-        cases (ks1 $k++ ks2 $? key_ref e); clean_map_lookups; eauto.
+    - case (k ==n x); intros; subst; clean_map_lookups;
+        progress_fold_add1; auto;
+          rewrite merge_perms_notation in *;
+          unfold add_key_perm in *.
+      + assert (ks1 $k++ ks2 $? x = None) by eauto.
+      context_map_rewrites; clean_map_lookups; auto.
+      + cases (ks1 $k++ ks2 $? x); clean_map_lookups; eauto.
   Qed.
+
+  Hint Resolve merge_perms_came_from_somewhere1 merge_perms_came_from_somewhere2.
 
   Lemma merge_perms_adds_ks1 :
     forall ks2 ks1 k v ks,
         ks1 $? k = Some v
       -> ks2 $? k = None
-      -> key_perms_good ks1                 
-      -> key_perms_good ks2
       -> ks = ks1 $k++ ks2
       -> ks $? k = Some v.
   Proof.
     unfold merge_perms.
-    induction ks2 using P.map_induction_bis; intros.
-
-    - apply map_eq_Equal in H; subst; eauto.
+    induction ks2 using P.map_induction_bis; intros; Equal_eq; eauto.
     - subst; rewrite fold_Empty; eauto.
     - case (x ==n k); intros; subst; clean_map_lookups; eauto.
       progress_fold_add1; auto.
       rewrite merge_perms_notation.
-      unfold add_key_perm_fold_fn, add_key_perm.
-      apply key_perms_good_add in H3; split_ands; subst; auto.
-      cases ( ks1 $k++ ks2 $? key_ref e ); clean_map_lookups; eauto.
+      unfold add_key_perm.
+      cases ( ks1 $k++ ks2 $? x ); clean_map_lookups; eauto.
   Qed.
 
   Lemma merge_perms_adds_ks2 :
     forall ks2 ks1 k v ks,
         ks1 $? k = None
       -> ks2 $? k = Some v
-      -> key_perms_good ks1                 
-      -> key_perms_good ks2
       -> ks = ks1 $k++ ks2
       -> ks $? k = Some v.
   Proof.
     unfold merge_perms.
-    induction ks2 using P.map_induction_bis; intros.
-    - apply map_eq_Equal in H; subst; eauto.
-    - invert H0.
-    - apply key_perms_good_add in H3; auto; split_ands; subst.
-      progress_fold_add1; auto.
-      rewrite merge_perms_notation.
-      unfold add_key_perm_fold_fn, add_key_perm.
-      cases (k ==n key_ref e); subst; clean_map_lookups.
-      + assert (ks1 $k++ ks2 $? key_ref v = None) as RW by eauto using merge_perms_adds_no_new_perms;
-          rewrite RW; clean_map_lookups; trivial.
-      + cases ( ks1 $k++ ks2 $? key_ref e); clean_map_lookups; eauto.
+    induction ks2 using P.map_induction_bis; intros; Equal_eq; contra_map_lookup; eauto.
+    subst; progress_fold_add1; auto.
+    rewrite merge_perms_notation.
+    unfold add_key_perm.
+    cases (k ==n x); subst; clean_map_lookups.
+    + assert (ks1 $k++ ks2 $? x = None) by eauto.
+      context_map_rewrites; clean_map_lookups; auto.
+    + cases ( ks1 $k++ ks2 $? x); clean_map_lookups; eauto.
   Qed.
+
+  Hint Resolve merge_perms_adds_ks1 merge_perms_adds_ks2.
+
+  Lemma merge_perms_chooses_greatest :
+    forall ks2 ks1 k k' kp kp',
+        ks1 $? k = Some kp
+      -> ks2 $? k' = Some kp'
+      -> k = k'
+      -> (ks1 $k++ ks2) $? k = Some (greatest_permission kp kp').
+  Proof.
+    induction ks2 using P.map_induction_bis; intros; Equal_eq; contra_map_lookup; eauto.
+    progress_fold_add1; auto.
+    rewrite merge_perms_notation.
+    unfold add_key_perm.
+    subst.
+    cases (x ==n k'); subst; clean_map_lookups.
+    + assert (ks1 $k++ ks2 $? k' = Some kp) by eauto.
+      context_map_rewrites; clean_map_lookups; auto.
+      rewrite greatest_permission_symm; trivial.
+    + cases (ks1 $k++ ks2 $? x); subst; clean_map_lookups; eauto.
+  Qed.
+
+  Hint Resolve merge_perms_chooses_greatest.
 
   Lemma merge_perms_split :
-    forall ks2 ks1 k,
-      ks1 $k++ ks2 $? key_ref k = Some k
-      -> key_perms_good ks1
-      -> key_perms_good ks2
-      -> ks1 $? key_ref k = Some k
-      \/ ks2 $? key_ref k = Some k.
+    forall ks2 ks1 k kp,
+      ks1 $k++ ks2 $? k = Some kp
+      -> ks1 $? k = Some kp
+      \/ ks2 $? k = Some kp.
   Proof.
-    induction ks2 using P.map_induction_bis; intros.
-    - apply map_eq_Equal in H; subst; auto.
-    - rewrite merge_keys_right_identity in H; auto.
-    - apply key_perms_good_add in H2; auto; split_ands; subst; clean_map_lookups.
-      cases (key_ref e ==n key_ref k).
-      + progress_fold_add1; auto. rewrite merge_perms_notation in H0.
-        unfold add_key_perm_fold_fn, add_key_perm in H0.
-        case_eq (ks1 $k++ ks2 $? key_ref e); intros; rewrite H2 in H0; clean_map_lookups; eauto.
-        rewrite e0 in H0; clean_map_lookups.
-        rewrite <- e0; clean_map_lookups.
-        unfold greatest_permission in *; destruct e; destruct k0; simpl in *.
-        cases has_private_access0; cases has_private_access1; simpl; auto.
-        pose proof (key_perms_merge_still_good H1 H3) as MERGE_GOOD.
-        assert (ks1 $k++ ks2 $? key_ref0 = Some {| key_ref := key_ref1; has_private_access := true |}) as EQ by assumption.
-        apply MERGE_GOOD in EQ; simpl in EQ; subst.
-        remember ({| key_ref := key_ref0; has_private_access := true |}) as k0.
-        assert (ks1 $k++ ks2 $? key_ref k0 = Some k0) as IND by (subst; simpl; auto).
-        specialize (IHks2 _ _ IND H1 H3); split_ors; subst.
-          intuition idtac.
-          simpl in *; contra_map_lookup.
-          rewrite add_eq_o by auto. rewrite add_eq_o in H0 by auto; intuition idtac.
-      + clean_map_lookups. apply IHks2; eauto.
-        progress_fold_add1; auto. rewrite merge_perms_notation in H0.
-        unfold add_key_perm_fold_fn, add_key_perm in H0; simpl in H0.
-        cases (ks1 $k++ ks2 $? key_ref e); clean_map_lookups; auto.
-  Qed.
+    induction ks2 using P.map_induction_bis; intros; Equal_eq; auto.
+    cases (x ==n k); subst; clean_map_lookups; auto;
+      progress_fold_add1; auto;
+        rewrite merge_perms_notation in *;
+        unfold add_key_perm in *.
 
-  Lemma key_perms_good_add_good_perm :
-    forall ks k,
-      key_perms_good ks
-      -> key_perms_good (ks $+ (key_ref k, k)).
-  Proof.
-    unfold key_perms_good; intros.
-    cases (key_ref k ==n k_id); subst; clean_map_lookups; auto.
-  Qed.
+    + subst. clean_map_lookups.
+      cases (ks1 $k++ ks2 $? k); clean_map_lookups; auto.
+      apply merge_perms_came_from_somewhere1 in Heq; auto.
+      unfold greatest_permission; cases e; cases b; simpl; auto.
 
-  Hint Resolve key_perms_good_add_good_perm.
+    + cases (ks1 $k++ ks2 $? x); clean_map_lookups; auto.
+  Qed.
 
   Lemma merge_perms_no_disappear_perms :
     forall ks2 k ks1,
-      (ks1 $k++ ks2) $? k = None
-    -> key_perms_good ks1
-    -> key_perms_good ks2
+      ks1 $k++ ks2 $? k = None
     -> ks1 $? k = None
     /\ ks2 $? k = None.
   Proof.
-    induction ks2 using P.map_induction_bis; intros; auto.
-    - apply map_eq_Equal in H; subst; auto.
+    induction ks2 using P.map_induction_bis; intros; Equal_eq; auto.
+    progress_fold_add1; auto.
+    rewrite merge_perms_notation in *; clean_map_lookups.
+    unfold add_key_perm in *.
+    cases (ks1 $k++ ks2 $? x);
+      cases (x ==n k); subst; clean_map_lookups; auto.
+  Qed.
+
+  Lemma merge_keys_neq_add_ok :
+    forall ks2 ks1 k k' kp,
+      k <> k'
+      -> ks1 $+ (k,kp) $k++ ks2 $? k' = ks1 $k++ ks2 $? k'.
+  Proof.
+    intros.
+    cases (ks1 $? k'); cases (ks2 $? k').
+    - erewrite !merge_perms_chooses_greatest; clean_map_lookups; eauto.
+    - erewrite !merge_perms_adds_ks1; auto; clean_map_lookups; eauto.
+    - erewrite !merge_perms_adds_ks2; auto; clean_map_lookups; eauto.
+    - erewrite !merge_perms_adds_no_new_perms; clean_map_lookups; auto.
+  Qed.
+
+  Hint Resolve merge_keys_neq_add_ok.
+
+  Lemma merge_keys_pull1 :
+    forall ks2 ks1 k kp kp' gkp,
+        ks2 $? k = Some kp'
+      -> gkp = greatest_permission kp kp'
+      -> (ks1 $+ (k, kp)) $k++ ks2 = ks1 $k++ ks2 $+ (k, gkp).
+  Proof.
+    induction ks2 using P.map_induction_bis; intros; Equal_eq; contra_map_lookup; eauto.
+    apply map_eq_Equal; unfold Equal; intros.
+    cases (k ==n x); cases (k ==n y); cases (x ==n y); subst; clean_map_lookups; try contradiction.
+    - eapply merge_perms_chooses_greatest; auto; clean_map_lookups; trivial.
+    - unfold merge_perms at 1; rewrite fold_add; auto; rewrite merge_perms_notation; unfold add_key_perm.
+      assert (ks1 $+ (x, kp) $k++ ks2 $? x = Some kp) by (eapply merge_perms_adds_ks1; eauto; clean_map_lookups; trivial).
+      context_map_rewrites; clean_map_lookups.
+      unfold merge_perms at 2; rewrite fold_add; auto; rewrite merge_perms_notation with (ks1:=ks1); unfold add_key_perm.
+      cases (ks1 $k++ ks2 $? x); subst; clean_map_lookups; eauto.
     - progress_fold_add1; auto.
-      rewrite merge_perms_notation in *; clean_map_lookups.
-      unfold add_key_perm_fold_fn, add_key_perm in H0.
-      apply key_perms_good_add in H2; split_ands; subst; auto.
-      cases (ks1 $k++ ks2 $? key_ref e); clean_map_lookups;
-        cases (key_ref e ==n k); subst; clean_map_lookups; auto.
-  Qed.
-
-
-  Lemma merge_keys_add_l_pull :
-    forall ks2 ks1 k,
-      ks2 $? key_ref k = None
-      -> key_perms_good ks1
-      -> key_perms_good ks2
-      -> ks1 $k++ ks2 $+ (key_ref k, k) = (ks1 $+ (key_ref k, k)) $k++ ks2.
-  Proof.
-    induction ks2 using P.map_induction_bis; auto; intros.
-    - apply map_eq_Equal in H; subst; auto.
-    - apply key_perms_good_add in H2; split_ands; subst; auto.
-      cases (key_ref e ==n key_ref k); try rewrite e0 in *; clean_map_lookups; auto.
-      unfold merge_perms at 2. rewrite fold_add; auto.
-      unfold add_key_perm_fold_fn at 1.
+      rewrite merge_perms_notation; unfold add_key_perm.
+      cases (ks1 $+ (y, kp) $k++ ks2 $? x); clean_map_lookups; auto;
+        erewrite merge_perms_chooses_greatest; auto; clean_map_lookups; eauto.
+    - unfold merge_perms; rewrite !fold_add; auto.
+      rewrite merge_perms_notation. rewrite merge_perms_notation with (ks1:=ks1).
       unfold add_key_perm.
-      rewrite merge_perms_notation with (ks1:=ks1 $+ (key_ref k, k)).
-      cases ( (ks1 $+ (key_ref k, k)) $k++ ks2 $? key_ref e); subst; clean_map_lookups; auto.
-      + rewrite <- IHks2; clean_map_lookups; auto.
-        unfold merge_perms at 1; rewrite fold_add; auto.
-        rewrite merge_perms_notation.
-        unfold add_key_perm_fold_fn, add_key_perm.
-        apply merge_perms_came_from_somewhere1 in Heq; auto.
-        clean_map_lookups.
-        assert (ks1 $k++ ks2 $? key_ref e = Some k0) as RW by (eauto using merge_perms_adds_ks1);
-          rewrite RW; clear RW.
-        apply map_eq_Equal; unfold Equal; intros.
-        cases (y ==n key_ref e); cases (y ==n key_ref k); subst; clean_map_lookups; trivial.
-      + rewrite <- IHks2; clean_map_lookups; auto.
-        unfold merge_perms at 1; rewrite fold_add; auto.
-        rewrite merge_perms_notation.
-        unfold add_key_perm_fold_fn, add_key_perm.
-        apply merge_perms_no_disappear_perms in Heq; auto; split_ands; clean_map_lookups.
-        assert (ks1 $k++ ks2 $? key_ref e = None) as RW by (eauto using merge_perms_adds_no_new_perms);
-          rewrite RW; clear RW.
-        apply map_eq_Equal; unfold Equal; intros.
-        cases (y ==n key_ref e); cases (y ==n key_ref k); subst; clean_map_lookups; trivial.
+      cases (ks1 $k++ ks2 $? y); eauto.
+      + assert (ks1 $? y = Some b) by eauto.
+        assert (ks1 $+ (k, kp) $k++ ks2 $? y = Some b). eapply merge_perms_adds_ks1; auto. clean_map_lookups; auto. auto.
+        context_map_rewrites; clean_map_lookups; trivial.
+      + eapply merge_perms_no_disappear_perms in Heq; auto; split_ands.
+        assert (ks1 $+ (k, kp) $k++ ks2 $? y = None) by (apply merge_perms_adds_no_new_perms; clean_map_lookups; auto).
+        context_map_rewrites; clean_map_lookups; auto.
+    - unfold merge_perms; rewrite !fold_add; auto.
+      rewrite merge_perms_notation. rewrite merge_perms_notation with (ks1:=ks1).
+      unfold add_key_perm.
+      cases (ks1 $k++ ks2 $? x); clean_map_lookups.
+      + apply merge_perms_came_from_somewhere1 in Heq; eauto.
+        assert (ks1 $+ (k, kp) $k++ ks2 $? x = Some b). eapply merge_perms_adds_ks1; auto. clean_map_lookups; auto. auto.
+        context_map_rewrites; clean_map_lookups; auto.
+      + eapply merge_perms_no_disappear_perms in Heq; auto; split_ands.
+        assert (ks1 $+ (k, kp) $k++ ks2 $? x = None) by (apply merge_perms_adds_no_new_perms; clean_map_lookups; auto).
+        context_map_rewrites; clean_map_lookups; auto.
   Qed.
 
-  Lemma merge_keys_add_l_pull_in :
-    forall ks2 ks1 k k',
-        ks2 $? key_ref k  = Some k'
-      -> ks1 $? key_ref k' = None
-      -> key_perms_good ks1
-      -> key_perms_good ks2
-      -> key_ref k = key_ref k'
-      -> ks1 $k++ ks2 $+ (key_ref k, greatest_permission k k') = (ks1 $+ (key_ref k, k)) $k++ ks2.
+  Lemma merge_keys_pull2 :
+    forall ks2 ks1 k kp gkp,
+        ks2 $? k = None
+      -> gkp = kp
+      -> (ks1 $+ (k, kp)) $k++ ks2 = ks1 $k++ ks2 $+ (k, gkp).
   Proof.
-    induction ks2 using P.map_induction_bis; auto; intros.
-    - apply map_eq_Equal in H; subst; auto.
-    - clean_map_lookups.
-    - apply key_perms_good_add in H3; split_ands; subst; auto.
-      cases (key_ref e ==n key_ref k'); try rewrite e0 in *; clean_map_lookups; auto.
-      + unfold merge_perms.
-        rewrite !fold_add; auto.
-        rewrite merge_perms_notation.
-        rewrite merge_perms_notation with (ks1:=ks1 $+ (key_ref k, k)).
-        cases (ks2 $? key_ref k).
-        * rewrite H4 in *; clean_map_lookups.
-        * rewrite <- merge_keys_add_l_pull; auto.
-          unfold add_key_perm_fold_fn, add_key_perm.
-          assert (ks1 $k++ ks2 $? key_ref k' = None) as RW by (eauto using merge_perms_adds_no_new_perms);
-            rewrite <- e0 in RW; rewrite RW; simpl; clean_map_lookups. rewrite e0,H4; clean_map_lookups.
-          rewrite H4 in H0; clean_map_lookups.
-          apply map_eq_Equal; unfold Equal; intros.
-          cases (key_ref k' ==n y); subst; clean_map_lookups; auto.
-          rewrite greatest_permission_symm; trivial.
-      + unfold merge_perms.
-        rewrite !fold_add; auto.
-        rewrite merge_perms_notation.
-        rewrite merge_perms_notation with (ks1:=ks1 $+ (key_ref k, k)).
-        rewrite H4 in H0; clean_map_lookups.
-        assert (key_ref e <> key_ref k) by (rewrite H4; assumption).
-        rewrite <- H4 in H0.
-        erewrite <- IHks2; eauto.
-        unfold add_key_perm_fold_fn, add_key_perm.
-        clean_map_lookups.
-        cases (ks1 $k++ ks2 $? key_ref e); subst; clean_map_lookups;
-          apply map_eq_Equal; unfold Equal; intros;
-            cases (y ==n key_ref e); cases (y ==n key_ref k); subst; clean_map_lookups; auto.
+    induction ks2 using P.map_induction_bis; intros; Equal_eq; autorewrite with core; subst; auto.
+    cases (x ==n k); subst; clean_map_lookups.
+    unfold merge_perms; rewrite !fold_add; auto.
+    rewrite merge_perms_notation. rewrite merge_perms_notation with (ks1:=ks1).
+    unfold add_key_perm.
+    cases (ks1 $k++ ks2 $? x).
+    - apply merge_perms_came_from_somewhere1 in Heq; auto.
+      assert (ks1 $+ (k, kp) $k++ ks2 $? x = Some b) by (eapply merge_perms_adds_ks1; trivial; clean_map_lookups; auto).
+      context_map_rewrites; clean_map_lookups; auto.
+      erewrite IHks2; auto.
+      apply map_eq_Equal; unfold Equal; intros.
+      cases (y ==n x); cases (y ==n k); subst; clean_map_lookups; auto; contradiction.
+    - apply merge_perms_no_disappear_perms in Heq; auto; split_ands.
+      assert (ks1 $+ (k, kp) $k++ ks2 $? x = None) by (apply merge_perms_adds_no_new_perms; clean_map_lookups; auto).
+      context_map_rewrites.
+      apply map_eq_Equal; unfold Equal; intros.
+      erewrite IHks2; auto.
+      cases (y ==n x); cases (y ==n k); subst; clean_map_lookups; auto; contradiction.
   Qed.
 
   Lemma merge_perms_sym :
     forall ks2 ks1,
-      key_perms_good ks1
-      -> key_perms_good ks2
-      -> ks1 $k++ ks2 = ks2 $k++ ks1.
+      ks1 $k++ ks2 = ks2 $k++ ks1.
   Proof.
-    induction ks2 using P.map_induction_bis; auto; intros.
-    - apply map_eq_Equal in H; subst; auto.
+    induction ks2 using P.map_induction_bis; intros; Equal_eq; eauto.
     - rewrite merge_keys_right_identity, merge_perms_left_identity; trivial.
-    - apply key_perms_good_add in H1; split_ands; subst; auto.
-      unfold merge_perms at 1; rewrite fold_add; auto.
+    - unfold merge_perms at 1; rewrite fold_add; auto.
       rewrite merge_perms_notation.
-      unfold add_key_perm_fold_fn, add_key_perm; simpl.
+      unfold add_key_perm; simpl.
 
-      cases (ks1 $k++ ks2 $? key_ref e); subst; clean_map_lookups.
+      cases (ks1 $k++ ks2 $? x); subst; clean_map_lookups.
       + apply merge_perms_came_from_somewhere1 in Heq; auto.
-        assert (key_ref k = key_ref e) by auto.
-        assert (ks2 $? key_ref k = None) by (rewrite H1; assumption).
-        rewrite IHks2 by auto.
-        erewrite <- merge_keys_add_l_pull_in; eauto.
+        erewrite merge_keys_pull1; eauto; rewrite IHks2; auto.
       + apply merge_perms_no_disappear_perms in Heq; auto; split_ands.
-        rewrite <- merge_keys_add_l_pull; auto.
-        rewrite IHks2; auto.
+        erewrite merge_keys_pull2; eauto; rewrite IHks2; auto.
   Qed.
 
   Lemma merge_perms_refl :
     forall ks,
-      key_perms_good ks
-      -> ks $k++ ks = ks.
+      ks $k++ ks = ks.
   Proof.
-    induction ks using P.map_induction_bis; auto.
-    - apply map_eq_Equal in H; subst; auto.
-    - unfold merge_perms; intros.
-      apply key_perms_good_add in H0; split_ands; subst; auto.
-      progress_fold_add1; auto.
-      rewrite merge_perms_notation.
-      unfold add_key_perm_fold_fn , add_key_perm.
-      rewrite <- merge_keys_add_l_pull; clean_map_lookups; auto.
-      rewrite IHks; auto.
-      apply map_eq_Equal; unfold Equal; intros.
-      cases (y ==n key_ref e); subst; clean_map_lookups; auto.
-      rewrite greatest_permission_refl; trivial.
+    induction ks using P.map_induction_bis; intros; Equal_eq; auto.
+    progress_fold_add1; auto.
+    rewrite merge_perms_notation.
+    unfold add_key_perm.
+    erewrite merge_keys_pull2; clean_map_lookups; auto.
+    rewrite map_add_eq, IHks; rewrite greatest_permission_refl; trivial.
   Qed.
-
-  Hint Extern 1 (key_perms_good (_ $k++ _)) => apply key_perms_merge_still_good.
-
-  Lemma merge_perms_chooses_greatest :
-    forall ks2 ks1 k k',
-      key_perms_good ks1
-      -> key_perms_good ks2
-      -> ks1 $? key_ref k = Some k
-      -> ks2 $? key_ref k' = Some k'
-      -> key_ref k = key_ref k'
-      -> (ks1 $k++ ks2) $? key_ref k = Some (greatest_permission k k').
-  Proof.
-    induction ks2 using P.map_induction_bis; intros; auto.
-    - apply map_eq_Equal in H; subst; auto.
-    - invert H2.
-    - apply key_perms_good_add in H1; split_ands; subst; auto.
-      progress_fold_add1; auto.
-      rewrite merge_perms_notation.
-      unfold add_key_perm_fold_fn, add_key_perm.
-      cases (key_ref e ==n key_ref k'); subst; try rewrite e0 in *; clean_map_lookups.
-      + rewrite H4 in H2.
-        assert (ks1 $k++ ks2 $? key_ref k' = Some k) as RW by eauto using merge_perms_adds_ks1;
-          rewrite RW; rewrite H4; clean_map_lookups.
-        rewrite greatest_permission_symm; auto.
-      + assert (key_ref e <> key_ref k) by (rewrite H4; assumption).
-        cases (ks1 $k++ ks2 $? key_ref e); subst; clean_map_lookups; eauto.
-  Qed.
-
-  Lemma merge_perms_assoc_helper :
-    forall ks1 ks2 k_id k_id' k k',
-      ks1 $k++ ks2 $? k_id = Some k
-      -> key_ref k = k_id
-      -> key_ref k' = k_id'
-      -> k_id <> k_id'
-      -> ks1 $k++ (ks2 $+ (k_id',k')) $? k_id = Some k.
-  Proof.
-  Admitted.
-
 
   Lemma merge_perms_assoc :
     forall ks3 ks1 ks2,
-      key_perms_good ks1
-      -> key_perms_good ks2
-      -> key_perms_good ks3
-      -> ks1 $k++ ks2 $k++ ks3 = ks1 $k++ (ks2 $k++ ks3).
+      ks1 $k++ ks2 $k++ ks3 = ks1 $k++ (ks2 $k++ ks3).
   Proof.
-    induction ks3 using P.map_induction_bis; intros; auto.
-    - apply map_eq_Equal in H; subst; auto.
-    - apply key_perms_good_add in H2; split_ands; subst; auto.
-      unfold merge_perms at 1.
-      unfold merge_perms at 3.
-      rewrite !fold_add; auto.
-      rewrite merge_perms_notation.
-      unfold add_key_perm_fold_fn at 1.
-      unfold add_key_perm_fold_fn at 1.
-      unfold add_key_perm.
-      rewrite merge_perms_notation with (ks1:=ks2).
+    induction ks3 using P.map_induction_bis; intros; Equal_eq; auto.
+    unfold merge_perms at 1.
+    unfold merge_perms at 3.
+    rewrite !fold_add; auto.
+    rewrite merge_perms_notation.
+    rewrite merge_perms_notation with (ks1:=ks2).
+    unfold add_key_perm.
 
-      cases (ks1 $k++ ks2 $k++ ks3 $? key_ref e);
-        cases (ks2 $k++ ks3 $? key_ref e); subst; clean_map_lookups;
-          rewrite IHks3 in Heq; auto.
-      + cases (ks1 $? key_ref e).
-        * assert (key_perms_good (ks1 $k++ (ks2 $k++ ks3))) as GD1 by eauto; specialize (GD1 _ _ Heq).
-          assert (key_perms_good (ks1)) as GD2 by eauto; specialize (GD2 _ _ Heq1).
-          assert (key_perms_good (ks2 $k++ ks3)) as GD3 by eauto; specialize (GD3 _ _ Heq0).
-          assert ( ks1 $k++ (ks2 $k++ ks3) $? key_ref k1 = Some (greatest_permission k1 k0) ).
-          eapply merge_perms_chooses_greatest; auto. rewrite GD2; auto. rewrite GD3; auto. rewrite GD2,GD3; trivial.
-          rewrite GD2 in H2. clean_map_lookups.
+    cases (ks2 $k++ ks3 $? x).
+    - cases (ks1 $k++ ks2 $k++ ks3 $? x);
+        subst; rewrite IHks3 in Heq0; clean_map_lookups; eauto.
+      + cases (ks1 $? x).
+        * assert (ks1 $k++ (ks2 $k++ ks3) $? x = Some (greatest_permission b1 b)) by eauto.
+          clean_map_lookups.
           apply map_eq_Equal; unfold Equal; intros.
-          cases (y ==n key_ref e); subst; clean_map_lookups.
-          ** symmetry. rewrite <- GD2 in Heq1.
-             rewrite <- GD2.
-             erewrite merge_perms_chooses_greatest with (k' := greatest_permission e k0); eauto;
-               destruct e; destruct k1; destruct k0; simpl in *; subst; simpl in *;
-                 unfold greatest_permission; simpl; auto.
-             rewrite !orb_assoc, orb_comm with (b1:= has_private_access1); trivial.
-             unfold key_perms_good; intros.
-             cases (key_ref0 ==n k_id); subst; clean_map_lookups; auto.
-             assert (key_perms_good (ks2 $k++ ks3)) by auto. specialize (H4 _ _ H2); eauto.
-             clean_map_lookups; trivial.
-          ** rewrite IHks3; auto.
-             cases (ks1 $k++ (ks2 $k++ ks3) $? y); symmetry.
-             *** assert (key_perms_good (ks1 $k++ (ks2 $k++ ks3))) as GD by auto; specialize (GD _ _ Heq2).
-                 apply merge_perms_assoc_helper; eauto.
-                 unfold greatest_permission; destruct e; destruct k0; simpl in *; eauto.
-             *** apply merge_perms_no_disappear_perms in Heq2; auto; split_ands.
-                 eapply merge_perms_adds_no_new_perms; clean_map_lookups; auto.
-                 unfold key_perms_good; intros.
-                 cases (k_id ==n key_ref e); subst; clean_map_lookups.
-                 unfold greatest_permission; destruct e; destruct k0; simpl in *; trivial.
-                 assert (key_perms_good (ks2 $k++ ks3)) by auto. specialize (H6 _ _ H5); eauto.
-
-        * apply merge_perms_came_from_somewhere2 in Heq; auto; clean_map_lookups.
+          cases (y ==n x); subst; clean_map_lookups.
+          ** assert (ks1 $k++ (ks2 $k++ ks3 $+ (x, greatest_permission e b)) $? x = Some (greatest_permission b1 (greatest_permission e b)))
+              by (eapply merge_perms_chooses_greatest; auto; clean_map_lookups; auto).
+             context_map_rewrites; unfold greatest_permission.
+             rewrite !orb_assoc, orb_comm with (b1:=e); trivial.
+          ** symmetry; rewrite merge_perms_sym.
+             rewrite merge_keys_neq_add_ok, merge_perms_sym, <- IHks3; auto; trivial.
+        * assert (ks1 $k++ (ks2 $k++ ks3) $? x = Some b) by eauto; clean_map_lookups.
           apply map_eq_Equal; unfold Equal; intros.
-          cases (y ==n key_ref e); subst; clean_map_lookups.
-          ** symmetry.
-             eapply merge_perms_adds_ks2 with (ks2 := ks2 $k++ ks3 $+ (key_ref e, greatest_permission e k0));
-               clean_map_lookups; eauto.
-             unfold key_perms_good; intros.
-             cases (k_id ==n key_ref e); subst; clean_map_lookups; eauto.
-             assert (key_perms_good (ks2 $k++ ks3)) as GD by eauto; specialize (GD _ _ Heq).
-             unfold greatest_permission; destruct e; destruct k0; simpl in *; trivial.
-             assert (key_perms_good (ks2 $k++ ks3)) as GD by eauto; specialize (GD _ _ H2); auto.
-          ** rewrite IHks3; auto.
-             cases (ks1 $k++ (ks2 $k++ ks3) $? y); symmetry.
-             *** assert (key_perms_good (ks1 $k++ (ks2 $k++ ks3))) as GD by auto; specialize (GD _ _ Heq0).
-                 apply merge_perms_assoc_helper; eauto.
-                 unfold greatest_permission; destruct e; destruct k0; simpl in *; eauto.
-             *** apply merge_perms_no_disappear_perms in Heq0; auto; split_ands.
-                 eapply merge_perms_adds_no_new_perms; clean_map_lookups; auto.
-                 unfold key_perms_good; intros.
-                 cases (k_id ==n key_ref e); subst; clean_map_lookups.
-                 unfold greatest_permission; destruct e; destruct k0; simpl in *; trivial.
-                 assert (key_perms_good (ks2 $k++ ks3)) by auto. specialize (H6 _ _ H5); eauto.
+          cases (y ==n x); subst; clean_map_lookups.
+          ** assert (ks1 $k++ (ks2 $k++ ks3 $+ (x, greatest_permission e b)) $? x = Some (greatest_permission e b))
+              by (eapply merge_perms_adds_ks2; auto; clean_map_lookups; auto).
+             context_map_rewrites; eauto.
+          ** symmetry; rewrite merge_perms_sym.
+             rewrite merge_keys_neq_add_ok, merge_perms_sym, <- IHks3; auto; trivial.
 
-      + unfold merge_perms at 3.
-        rewrite fold_add; auto.
-        rewrite merge_perms_notation with (ks2:=ks2 $k++ ks3).
-        unfold add_key_perm_fold_fn, add_key_perm.
-        rewrite Heq.
-        rewrite IHks3; auto.
-      + apply merge_perms_no_disappear_perms in Heq; auto; split_ands; contra_map_lookup.
+      + apply merge_perms_no_disappear_perms in Heq0; auto; split_ands; contra_map_lookup.
 
-      + unfold merge_perms at 3.
-        rewrite fold_add; auto.
-        rewrite merge_perms_notation with (ks2:=ks2 $k++ ks3).
-        unfold add_key_perm_fold_fn, add_key_perm.
-        rewrite Heq.
-        rewrite IHks3; auto.
+    - unfold merge_perms at 7.
+      rewrite fold_add; auto.
+      unfold add_key_perm at 1. rewrite merge_perms_notation with (ks2:=ks2 $k++ ks3).
+      rewrite IHks3; trivial.
   Qed.
 
-  Lemma merge_perm_heaps_proper :
+  Lemma findUserKeys_foldfn_proper :
     forall {A},
       Proper (eq ==> eq ==> eq ==> eq) (fun (_ : NatMap.key) (u : user_data A) (ks : key_perms) => ks $k++ key_heap u).
   Proof.
     unfold Proper, respectful; intros; subst; trivial.
   Qed.
 
-  Lemma merge_perm_heaps_transpose :
+  Lemma findUserKeys_foldfn_transpose :
     forall {A},
       transpose_neqkey eq (fun (_ : NatMap.key) (u : user_data A) (ks : key_perms) => ks $k++ key_heap u).
   Proof.
     unfold transpose_neqkey; intros.
-    rewrite !merge_perms_assoc, merge_perms_sym with (ks1:= key_heap e'); trivial.
-
-  Admitted.
-
-
-
-
-
-  Lemma findKeys_good :
-    forall {t} (msg : message t),
-      key_perms_good (findKeys msg).
-  Proof.
-    induction msg; intros; simpl in *; subst; eauto using key_perms_merge_still_good.
+    rewrite !merge_perms_assoc,merge_perms_sym with (ks1:=key_heap e'); trivial.
   Qed.
 
-  Definition all_user_key_perms_good {A} (usrs : honest_users A) :=
-    forall u_id u_d, usrs $? u_id = Some u_d -> key_perms_good u_d.(key_heap).
+  Hint Resolve findUserKeys_foldfn_proper findUserKeys_foldfn_transpose.
 
-  Lemma findUserKeys_result_perms_good :
+  Lemma findUserKeys_notation :
     forall {A} (usrs : honest_users A),
-        all_user_key_perms_good usrs
-      -> key_perms_good (findUserKeys usrs).
-  Proof.
-    unfold all_user_key_perms_good, findUserKeys; intros.
-    apply P.fold_rec_bis; auto; intros.
-    apply find_mapsto_iff in H0.
-    apply key_perms_merge_still_good; eauto.
+      fold (fun (_ : NatMap.key) (u : user_data A) (ks : key_perms) => ks $k++ key_heap u) usrs $0 = findUserKeys usrs.
+    unfold findUserKeys; trivial.
   Qed.
 
-  (* Lemma findUserKeys_as_map_fold : *)
-  (*   forall {A} (usrs : honest_users A), *)
-  (*     all_user_key_perms_good usrs *)
-  (*     -> findUserKeys usrs = fold (fun _ => merge_perms) (map (@key_heap A) usrs) $0. *)
-  (* Proof. *)
-  (*   unfold findUserKeys; intros. *)
-  (*   apply P.fold_rec_bis; intros; subst; eauto. *)
-  (*   - apply map_eq_Equal in H0; subst; auto. *)
-  (*   - admit. *)
-  (* Admitted. *)
+  Lemma map_ne_swap :
+    forall {V} (m : NatMap.t V) k v k' v',
+      k <> k'
+      -> m $+ (k,v) $+ (k',v') = m $+ (k',v') $+ (k,v).
+  Proof.
+    intros.
+    apply map_eq_Equal; unfold Equal; intros.
+    cases (y ==n k); cases (y ==n k'); subst; clean_map_lookups; auto; contradiction.
+  Qed.
 
   Lemma findUserKeys_readd_user_same_keys_idempotent :
     forall {A} (usrs : honest_users A) u_id u_d proto msgs,
       usrs $? u_id = Some u_d
-      -> all_user_key_perms_good usrs
-      -> key_perms_good (findUserKeys usrs)
       -> findUserKeys usrs = findUserKeys (usrs $+ (u_id, {| key_heap := key_heap u_d; protocol := proto; msg_heap := msgs |})).
   Proof.
     intros.
-    unfold findUserKeys; generalize H H0 H1.
-    apply P.fold_rec_bis; intros; subst.
-    - apply map_eq_Equal in H2; subst; auto.
-    - invert H2.
-    - unfold all_user_key_perms_good in H6.
-      assert (key_perms_good (key_heap e)) by (eapply H6 with (u_id := k); clean_map_lookups; auto).
-      cases (k ==n u_id); subst; clean_map_lookups.
+    induction usrs using P.map_induction_bis; intros; Equal_eq; contra_map_lookup; auto.
 
-  Admitted.
-
+    cases (x ==n u_id); subst; clean_map_lookups.
+    - rewrite map_add_eq.
+      unfold findUserKeys.
+      rewrite !fold_add; auto.
+    - rewrite map_ne_swap; auto.
+      unfold findUserKeys.
+      rewrite fold_add; auto.
+      rewrite fold_add; auto; clean_map_lookups.
+      rewrite !findUserKeys_notation.
+      rewrite IHusrs at 1; auto.
+      rewrite not_find_in_iff; clean_map_lookups; trivial.
+  Qed.
 
   Lemma safe_messages_have_no_bad_keys :
     forall {t} (msg : message t) msgk,
@@ -1132,462 +910,14 @@ Section KeyMergeTheorems.
 
     - destruct k; simpl in *.
       unfold honest_key.
-      cases (key_ref0 ==n k_id); subst; clean_map_lookups.
+      cases (k ==n k_id); subst; clean_map_lookups.
       cases (all_keys $? k_id); eauto.
       destruct k.
-      specialize (k_good _ Heq); simpl in k_good; subst.
-      unfold honest_key in *. rewrite Heq in H.
+      unfold honest_key in *; context_map_rewrites.
       cases keyType0; eauto.
     - apply orb_false_elim in H; split_ands.
-      assert (key_perms_good (findKeys msg1 $k++ findKeys msg2)) as FIND by eauto using findKeys_good, key_perms_merge_still_good.
-      assert (findKeys msg1 $k++ findKeys msg2 $? k_id = Some k) as KID by assumption.
-      apply FIND in KID; rewrite <- KID in H2.
-      apply merge_perms_split in H2; eauto using findKeys_good.
-      split_ors; eauto.
+      apply merge_perms_split in H2; auto; split_ors; eauto.
   Qed.
-
-  (* Definition key_heaps_compatible (ks1 ks2 : keys) := *)
-  (*     keys_good ks1 *)
-  (*   /\ keys_good ks2 *)
-  (*   /\ (forall k_id k k', ks1 $? k_id = Some k -> ks2 $? k_id = Some k' -> keys_compatible k k' = true). *)
-
-  (* Lemma canonical_key_one_other : *)
-  (*   forall k1 k2, *)
-  (*       canonical_key k1 k2 = k1 *)
-  (*     \/ canonical_key k1 k2 = k2. *)
-  (* Proof. *)
-  (*   intros; unfold canonical_key. *)
-  (*   destruct k1; destruct k2; simpl. *)
-  (*   cases (keyId0 ?= keyId1); *)
-  (*     cases keyUsage0; cases keyUsage1; *)
-  (*       cases keyType0; cases keyType1; eauto; *)
-  (*         try rewrite Nat.compare_refl; simpl; eauto; *)
-  (*           cases has_private_access; cases has_private_access0; eauto. *)
-  (* Qed. *)
-
-  (* Lemma canonical_key_refl : *)
-  (*   forall k, canonical_key k k = k. *)
-  (* Proof. *)
-  (*   unfold canonical_key; intros; simpl. *)
-  (*   rewrite Nat.compare_refl. *)
-  (*   cases (keyUsage k); cases (keyType k); simpl; eauto; cases has_private_access; eauto. *)
-  (* Qed. *)
-
-  (* Lemma canonical_key_sym : *)
-  (*   forall k1 k2, *)
-  (*     canonical_key k1 k2 = canonical_key k2 k1. *)
-  (* Proof. *)
-  (*   intros; destruct k1; destruct k2; unfold canonical_key; simpl. *)
-  (*   cases (keyId0 ?= keyId1). *)
-  (*   - apply Nat.compare_eq in Heq; subst. *)
-  (*     rewrite Nat.compare_refl. *)
-  (*     cases keyUsage0; cases keyUsage1; cases keyType0; cases keyType1; eauto. *)
-  (*     cases has_private_access; cases has_private_access0; eauto. *)
-  (*     cases has_private_access; cases has_private_access0; eauto. *)
-
-  (*   - rewrite Nat.compare_antisym; rewrite Heq; simpl; auto. *)
-  (*   - rewrite Nat.compare_antisym; rewrite Heq; simpl; auto. *)
-  (* Qed. *)
-
-  (* Lemma canonical_key_assoc : *)
-  (*   forall k1 k2 k3, *)
-  (*     canonical_key k1 (canonical_key k2 k3) = canonical_key (canonical_key k1 k2) k3. *)
-  (* Proof. *)
-  (*   intros; destruct k1; destruct k2; destruct k3; unfold canonical_key; simpl. *)
-
-  (*   cases (keyId0 ?= keyId1); cases (keyId1 ?= keyId2). *)
-  (*   - apply Nat.compare_eq in Heq; apply Nat.compare_eq in Heq0; subst. simpl. *)
-  (*     cases keyUsage0; cases keyUsage1; cases keyUsage2; *)
-  (*       cases keyType0; cases keyType1; cases keyType2; *)
-  (*         simpl; eauto; *)
-  (*           try rewrite Nat.compare_refl; eauto; *)
-  (*             cases has_private_access; cases has_private_access0; try cases has_private_access1; simpl; *)
-  (*               try rewrite Nat.compare_refl; eauto. *)
-
-  (*   - apply Nat.compare_eq in Heq; subst; simpl. *)
-  (*     rewrite Heq0; simpl. *)
-  (*     cases keyUsage0; cases keyUsage1; cases keyUsage2; *)
-  (*       cases keyType0; cases keyType1; cases keyType2; *)
-  (*         simpl; eauto; try rewrite Heq0; simpl; eauto; *)
-  (*           cases has_private_access; cases has_private_access0; try cases has_private_access1; simpl; *)
-  (*             rewrite Heq0; simpl; eauto. *)
-
-  (*   - apply Nat.compare_eq in Heq; subst; simpl. *)
-  (*     rewrite Nat.compare_refl. *)
-  (*     cases keyUsage0; cases keyUsage1; cases keyUsage2; *)
-  (*       cases keyType0; cases keyType1; cases keyType2; *)
-  (*         simpl; eauto; try rewrite Heq0; simpl; eauto; *)
-  (*           cases has_private_access; cases has_private_access0; try cases has_private_access1; simpl; *)
-  (*             rewrite Heq0; simpl; eauto. *)
-
-  (*   - apply Nat.compare_eq in Heq0; subst; simpl. *)
-  (*     rewrite Nat.compare_refl; simpl. *)
-  (*     cases keyUsage0; cases keyUsage1; cases keyUsage2; *)
-  (*       cases keyType0; cases keyType1; cases keyType2; *)
-  (*         simpl; eauto; try rewrite Heq; simpl; eauto; *)
-  (*           cases has_private_access; cases has_private_access0; try cases has_private_access1; simpl; *)
-  (*             rewrite Heq; simpl; eauto. *)
-
-  (*   - simpl. rewrite Heq0. *)
-  (*     pose proof Heq as lt1; pose proof Heq0 as lt2. *)
-  (*     apply nat_compare_lt in lt1; apply nat_compare_lt in lt2. *)
-  (*     pose proof (Nat.lt_trans _ _ _ lt1 lt2). apply nat_compare_lt in H. *)
-  (*     rewrite H; eauto. *)
-
-  (*   - simpl; rewrite Heq; rewrite Heq0; eauto. *)
-
-  (*   - apply Nat.compare_eq in Heq0; subst; simpl. *)
-  (*     rewrite Heq; simpl. *)
-  (*     cases keyUsage0; cases keyUsage1; cases keyUsage2; *)
-  (*       cases keyType0; cases keyType1; cases keyType2; *)
-  (*         simpl; eauto; try rewrite Heq; simpl; eauto; *)
-  (*           cases has_private_access; cases has_private_access0; try cases has_private_access1; simpl; *)
-  (*             rewrite Heq; simpl; eauto. *)
-
-  (*   - simpl. cases (keyId0 ?= keyId2); simpl; eauto. *)
-  (*   - simpl. rewrite Heq. *)
-  (*     pose proof Heq as gt1; pose proof Heq0 as gt2. *)
-  (*     apply nat_compare_gt in gt1; apply nat_compare_gt in gt2. *)
-
-  (*     pose proof (gt_trans _ _ _ gt1 gt2); apply nat_compare_gt in H. *)
-  (*     rewrite H; simpl; eauto. *)
-  (* Qed. *)
-
-  (* Lemma merge_keys_fold_fn_proper : *)
-  (*     Morphisms.Proper *)
-  (*       (Morphisms.respectful eq (Morphisms.respectful eq (Morphisms.respectful eq eq))) *)
-  (*       add_key. *)
-  (* Proof. *)
-  (*   unfold Morphisms.Proper, Morphisms.respectful; intros; simpl; subst; trivial. *)
-  (* Qed. *)
-
-  (* Lemma merge_keys_fold_fn_proper_flip : *)
-  (*     Morphisms.Proper *)
-  (*       (Morphisms.respectful eq (Morphisms.respectful eq (Morphisms.respectful (Basics.flip eq) (Basics.flip eq)))) *)
-  (*       add_key. *)
-  (* Proof. *)
-  (*   unfold Morphisms.Proper, Morphisms.respectful; intros; simpl; unfold Basics.flip in *; subst; trivial. *)
-  (* Qed. *)
-
-  (* Lemma merge_keys_fold_fn_proper_Equal : *)
-  (*   Morphisms.Proper *)
-  (*     (Morphisms.respectful eq (Morphisms.respectful eq (Morphisms.respectful Equal Equal))) *)
-  (*     add_key. *)
-  (* Proof. *)
-  (*   unfold Morphisms.Proper, Morphisms.respectful; intros; simpl; subst. *)
-  (*   apply map_eq_Equal in H1; subst. *)
-  (*   apply Equal_refl. *)
-  (* Qed. *)
-
-  (* Lemma merge_keys_transpose : *)
-  (*   transpose_neqkey eq add_key. *)
-  (* Proof. *)
-  (*   unfold transpose_neqkey; intros. *)
-  (*   unfold add_key; simpl. *)
-  (*   case_eq (a $? k); case_eq (a $? k'); intros; subst; simpl. *)
-
-  (*   Ltac work1 := *)
-  (*     match goal with *)
-  (*     | [ H : ?x <> ?x |- _ ] => contradiction *)
-  (*     | [ H1 : ?x <> ?y, H2 : ?x = ?y |- _ ] => contradiction *)
-  (*     | [ H : ?a $? ?k  = _ |- context [?a $? ?k]  ] => rewrite H *)
-  (*     | [ H : ?a $? ?k' = _ |- context [?a $? ?k'] ] => rewrite H *)
-  (*     | [ |- context[ ?k1 ==kk ?k2 ] ] => case (k1 ==kk k2); intros; subst *)
-  (*     | [ H : keys_compatible ?k1 ?k2 = _ |- context [ keys_compatible ?k1 ?k2 ]] => rewrite H *)
-  (*     | [ |- context [ keys_compatible ?k1 ?k2 ]] => case_eq (keys_compatible k1 k2); intros *)
-  (*     | [ H : keyType ?k = _ |- context [ keyType ?k ==kt ?kt ]] => rewrite H *)
-  (*     | [ |- context [ keyType ?k ==kt ?kt ]] => case (keyType k ==kt kt); intros *)
-  (*     | [ |- context [ _ $+ (?k1, _) $? ?k1 ]] => rewrite add_eq_o by (trivial || auto) *)
-  (*     | [ |- context [ _ $+ (?k1, _) $? ?k2 ]] => rewrite add_neq_o by auto *)
-  (*     | [ |- context [ _ $- ?k1 $? ?k2 ]] => rewrite remove_neq_o by auto *)
-  (*     end. *)
-
-  (*   Ltac maps_equal := *)
-  (*     repeat match goal with *)
-  (*            | [ |- context[find ?k (add ?k _ _) ] ]  => rewrite add_eq_o by auto *)
-  (*            | [ |- context[find ?k (add ?k' _ _) ] ] => rewrite add_neq_o by auto *)
-  (*            | [ |- context[find ?k (remove ?k _) ] ]  => rewrite remove_eq_o by auto *)
-  (*            | [ |- context[find ?k (remove ?k' _) ] ] => rewrite remove_neq_o by auto *)
-  (*            | [ |- _ $+ (?k1,_) $? ?k = _ ] => case (k1 ==n k); intros; subst *)
-  (*            | [ |- _ $- ?k1     $? ?k = _ ] => case (k1 ==n k); intros; subst *)
-  (*            | [ |- add _ _ _ = _ ] => apply map_eq_Equal; unfold Equal; intros ?y *)
-  (*            end. *)
-
-  (*   repeat work1; eauto; *)
-  (*     apply map_eq_Equal; unfold Equal; intros; *)
-  (*       maps_equal; auto. *)
-    
-  (*   repeat work1; eauto; *)
-  (*     apply map_eq_Equal; unfold Equal; intros; *)
-  (*       maps_equal; auto. *)
-
-  (*   repeat work1; eauto; *)
-  (*     apply map_eq_Equal; unfold Equal; intros; *)
-  (*       maps_equal; auto. *)
-
-  (*   repeat work1; eauto; *)
-  (*     apply map_eq_Equal; unfold Equal; intros; *)
-  (*       maps_equal; auto. *)
-
-  (* Qed. *)
-
-  (* Lemma merge_keys_transpose_flip : *)
-  (*   transpose_neqkey (Basics.flip eq) add_key. *)
-  (* Proof. *)
-  (*   unfold transpose_neqkey, Basics.flip; intros. *)
-  (*   apply merge_keys_transpose; auto. *)
-  (* Qed. *)
-
-  (* Lemma eq_Equal : *)
-  (*   forall {V} (m m' : NatMap.t V), *)
-  (*     m = m' *)
-  (*     -> Equal m m'. *)
-  (*   intros; subst; apply Equal_refl. *)
-  (* Qed. *)
-
-  (* Lemma merge_keys_transpose_Equal : *)
-  (*   transpose_neqkey Equal add_key. *)
-  (* Proof. *)
-  (*   unfold transpose_neqkey; intros. *)
-  (*   apply eq_Equal. *)
-  (*   apply merge_keys_transpose; auto. *)
-  (* Qed. *)
-
-  (* Hint Resolve merge_keys_fold_fn_proper merge_keys_fold_fn_proper_flip merge_keys_fold_fn_proper_Equal *)
-  (*              merge_keys_transpose merge_keys_transpose_flip merge_keys_transpose_Equal. *)
-
-  (* Lemma merge_keys_left_identity : *)
-  (*   forall ks, *)
-  (*     $0 $k++ ks = ks. *)
-  (* Proof. *)
-  (*   unfold merge_keys. *)
-  (*   induction ks using P.map_induction_bis; intros. *)
-
-  (*   - apply map_eq_Equal in H; subst; auto. *)
-  (*   - apply fold_Empty; eauto. *)
-  (*   - rewrite fold_add; clean_map_lookups; eauto. *)
-  (*     rewrite IHks; clear IHks. *)
-  (*     unfold add_key; rewrite H; eauto. *)
-  (* Qed. *)
-
-  (* Lemma merge_keys_right_identity : *)
-  (*   forall ks, *)
-  (*     ks $k++ $0 = ks. *)
-  (* Proof. *)
-  (*   unfold merge_keys; intros; rewrite fold_Empty; eauto. *)
-  (* Qed. *)
-
-  (* Hint Resolve merge_keys_left_identity merge_keys_right_identity. *)
-
-  (* Lemma merge_keys_adds_no_new_keys : *)
-  (*   forall ks2 k ks1, *)
-  (*       ks1 $? k = None *)
-  (*     -> ks2 $? k = None *)
-  (*     -> (ks1 $k++ ks2) $? k = None. *)
-  (* Proof. *)
-  (*   induction ks2 using P.map_induction_bis; intros. *)
-  (*   - apply map_eq_Equal in H; subst; auto. *)
-  (*   - rewrite merge_keys_right_identity; auto. *)
-  (*   - unfold merge_keys; rewrite fold_add; auto. *)
-  (*     case (x ==n k); intros; subst; clean_map_lookups. *)
-  (*     + rewrite merge_keys_notation; unfold add_key. *)
-  (*       cases (ks1 $k++ ks2 $? x); clean_map_lookups; eauto. *)
-  (*       cases (e ==kk k0); subst; eauto. *)
-  (*       clean_map_lookups. eapply IHks2; auto. *)
-  (* Qed. *)
-
-  (* Lemma merge_keys_no_disappear_keys : *)
-  (*   forall ks2 k ks1, *)
-  (*     (ks1 $k++ ks2) $? k = None *)
-  (*   -> ks1 $? k = None *)
-  (*   /\ ks2 $? k = None. *)
-  (* Proof. *)
-  (*   induction ks2 using P.map_induction_bis; intros. *)
-  (*   - apply map_eq_Equal in H; subst; auto. *)
-  (*   - rewrite merge_keys_right_identity in H; eauto. *)
-  (*   - unfold merge_keys in H0. progress_fold_add1; auto. *)
-  (*     rewrite merge_keys_notation in *; clean_map_lookups. *)
-  (*     unfold add_key in H0. *)
-  (*     cases (ks1 $k++ ks2 $? x); clean_map_lookups; *)
-  (*       [cases (e ==kk k0); subst | ]; *)
-  (*         case (x ==n k); intros; subst; clean_map_lookups; eauto. *)
-  (* Qed. *)
-
-  (* Hint Resolve merge_keys_adds_no_new_keys merge_keys_no_disappear_keys. *)
-
-  (* Lemma merge_keys_adds_ks1 : *)
-  (*   forall ks2 ks1 k v ks, *)
-  (*       ks1 $? k = Some v *)
-  (*     -> ks2 $? k = None *)
-  (*     -> ks = ks1 $k++ ks2 *)
-  (*     -> ks $? k = Some v. *)
-  (* Proof. *)
-  (*   unfold merge_keys. *)
-  (*   induction ks2 using P.map_induction_bis; intros. *)
-
-  (*   - apply map_eq_Equal in H; subst; eauto. *)
-  (*   - subst; rewrite fold_Empty; eauto. *)
-  (*   - case (x ==n k); intros; subst; clean_map_lookups; eauto. *)
-  (*     rewrite fold_add; eauto. *)
-  (*     rewrite merge_keys_notation. *)
-  (*     unfold add_key. *)
-  (*     cases ( ks1 $k++ ks2 $? x ); clean_map_lookups; eauto. *)
-  (*     cases ( e ==kk k0 ); eauto. *)
-  (*     clean_map_lookups; eauto. *)
-  (* Qed. *)
-
-  (* Lemma merge_keys_adds_ks2 : *)
-  (*   forall ks2 ks1 k v ks, *)
-  (*       ks1 $? k = None *)
-  (*     -> ks2 $? k = Some v *)
-  (*     -> ks = ks1 $k++ ks2 *)
-  (*     -> ks $? k = Some v. *)
-  (* Proof. *)
-  (*   unfold merge_keys. *)
-  (*   induction ks2 using P.map_induction_bis; intros. *)
-
-  (*   - apply map_eq_Equal in H; subst; eauto. *)
-  (*   - invert H0. *)
-  (*   - subst. *)
-  (*     case (x ==n k); intros; subst; clean_map_lookups; eauto. *)
-  (*     + rewrite fold_add; auto. *)
-  (*       rewrite merge_keys_notation. *)
-  (*       unfold add_key. *)
-  (*       pose proof merge_keys_adds_no_new_keys. *)
-  (*       cases ( ks1 $k++ ks2 $? k); clean_map_lookups; eauto. *)
-  (*       cases ( v ==kk k0 ); subst; clean_map_lookups; eauto. *)
-  (*       specialize (H1 _ _ _ H0 H); contra_map_lookup. *)
-
-  (*     + rewrite fold_add; auto. *)
-  (*       rewrite merge_keys_notation. *)
-  (*       unfold add_key. *)
-  (*       cases ( ks1 $k++ ks2 $? x); clean_map_lookups; eauto. *)
-  (*       cases ( e ==kk k0 ); eauto. *)
-  (*       clean_map_lookups; eauto. *)
-  (* Qed. *)
-
-  (* Hint Resolve merge_keys_adds_ks1 merge_keys_adds_ks2. *)
-
-  (* Lemma merge_keys_came_from_somewhere1 : *)
-  (*   forall ks2 ks1 k v, *)
-  (*       ks1 $k++ ks2 $? k = Some v *)
-  (*     -> ks2 $? k = None *)
-  (*     -> ks1 $? k = Some v. *)
-  (* Proof. *)
-  (*   unfold merge_keys. *)
-  (*   induction ks2 using P.map_induction_bis; intros. *)
-
-  (*   - apply map_eq_Equal in H; subst; eauto. *)
-  (*   - rewrite fold_Empty in H; auto. *)
-
-  (*   - case (x ==n k); intros; subst; clean_map_lookups. *)
-  (*     + progress_fold_add1; auto. *)
-  (*       rewrite merge_keys_notation in H0; unfold add_key at 1 in H0. *)
-
-  (*       cases (ks1 $k++ ks2 $? x); clean_map_lookups; eauto. *)
-  (*       cases ( e ==kk k0 ); subst; clean_map_lookups; eauto. *)
-  (* Qed. *)
-
-  (* Lemma merge_keys_came_from_somewhere2 : *)
-  (*   forall ks2 ks1 k v, *)
-  (*       ks1 $k++ ks2 $? k = Some v *)
-  (*     -> ks1 $? k = None *)
-  (*     -> ks2 $? k = Some v. *)
-  (* Proof. *)
-  (*   unfold merge_keys. *)
-  (*   induction ks2 using P.map_induction_bis; intros. *)
-
-  (*   - apply map_eq_Equal in H; subst; eauto. *)
-  (*   - rewrite fold_Empty in H; clean_map_lookups; auto. *)
-
-  (*   - case (x ==n k); intros; subst; clean_map_lookups; progress_fold_add1; auto. *)
-  (*     * pose proof (merge_keys_adds_no_new_keys _ _ _ H1 H). *)
-  (*       rewrite merge_keys_notation in H0; unfold add_key in H0; auto. *)
-  (*       cases (ks1 $k++ ks2 $? k); clean_map_lookups; eauto. *)
-
-  (*     * rewrite merge_keys_notation in H0; unfold add_key in H0; auto. *)
-  (*       cases (ks1 $k++ ks2 $? x); clean_map_lookups; eauto. *)
-  (*       cases ( e ==kk k0 ); subst; clean_map_lookups; eauto. *)
-  (* Qed. *)
-
-  (* Hint Resolve merge_keys_came_from_somewhere1 merge_keys_came_from_somewhere2. *)
-
-  (* Lemma merge_keys_split : *)
-  (*   forall ks2 k_id k ks1, *)
-  (*     ks1 $k++ ks2 $? k_id = Some k *)
-  (*     -> (ks1 $? k_id = None /\ ks2 $? k_id = Some k) *)
-  (*     \/ (ks1 $? k_id = Some k /\ ks2 $? k_id = None) *)
-  (*     \/ exists k1 k2, ks1 $? k_id = Some k1 /\ ks2 $? k_id = Some k2 /\ k = canonical_key k1 k2. *)
-  (* Proof. *)
-  (*   unfold merge_keys. *)
-  (*   induction ks2 using P.map_induction_bis; intros. *)
-  (*   - apply map_eq_Equal in H; subst; eauto. *)
-  (*   - rewrite merge_keys_right_identity in H. intuition idtac. *)
-  (*   - rewrite fold_add in H0; auto. *)
-  (*     rewrite merge_keys_notation in H0; unfold add_key in H0; auto. *)
-  (*     case (x ==n k_id); intros; subst; clean_map_lookups. *)
-  (*     + cases (ks1 $k++ ks2 $? k_id); intros; simpl. *)
-  (*       * cases (e ==kk k0); subst. *)
-  (*         ** rewrite Heq in H0; invert H0. eapply merge_keys_came_from_somewhere1 in Heq; auto. *)
-  (*            right; right. do 2 eexists; intuition eauto. rewrite canonical_key_refl; trivial. *)
-  (*         ** clean_map_lookups; eapply merge_keys_came_from_somewhere1 in Heq; auto. *)
-  (*            right; right; do 2 eexists; intuition eauto. rewrite canonical_key_sym; trivial. *)
-
-  (*       * clean_map_lookups; eauto. eapply merge_keys_no_disappear_keys in Heq; invert Heq. *)
-  (*         intuition idtac. *)
-  (*     + cases (ks1 $k++ ks2 $? x); clean_map_lookups; eauto. *)
-  (*       cases (e ==kk k0); auto. *)
-  (*       cases (x ==n k_id); clean_map_lookups; auto. *)
-  (* Qed. *)
-
-  (* Lemma merge_keys_canonicalizes : *)
-  (*   forall ks2 k_id k k1 k2 ks1, *)
-  (*       ks1 $k++ ks2 $? k_id = Some k *)
-  (*     -> ks1 $? k_id = Some k1 *)
-  (*     -> ks2 $? k_id = Some k2 *)
-  (*     -> k = canonical_key k1 k2. *)
-  (* Proof. *)
-  (*   unfold merge_keys. *)
-  (*   induction ks2 using P.map_induction_bis; intros. *)
-  (*   - apply map_eq_Equal in H; subst; eauto. *)
-  (*   - invert H1. *)
-
-  (*   - rewrite fold_add in H0; auto. *)
-  (*     rewrite merge_keys_notation in H0; unfold add_key in H0; auto. *)
-  (*     case (x ==n k_id); intros; subst; clean_map_lookups. *)
-  (*     + cases (ks1 $k++ ks2 $? k_id); intros; simpl. *)
-  (*       * cases (k2 ==kk k0); subst; eauto. *)
-  (*         ** rewrite Heq in H0; invert H0. eapply merge_keys_came_from_somewhere1 in Heq; auto. rewrite Heq in H1; invert H1. rewrite canonical_key_refl; trivial. *)
-  (*         ** clean_map_lookups. eapply merge_keys_came_from_somewhere1 in Heq; auto. rewrite Heq in H1; invert H1. rewrite canonical_key_sym; trivial. *)
-
-  (*       * clean_map_lookups. eapply merge_keys_no_disappear_keys in Heq; destruct Heq; contra_map_lookup. *)
-
-  (*     + cases (ks1 $k++ ks2 $? x); clean_map_lookups; eauto. *)
-  (*       cases (e ==kk k0); subst; clean_map_lookups; eauto. *)
-  (* Qed. *)
-
-  (* Lemma merge_keys_canonicalizes' : *)
-  (*   forall ks2 k_id k k1 k2 ks1, *)
-  (*       ks1 $? k_id = Some k1 *)
-  (*     -> ks2 $? k_id = Some k2 *)
-  (*     -> k = canonical_key k1 k2 *)
-  (*     -> ks1 $k++ ks2 $? k_id = Some k. *)
-  (* Proof. *)
-  (*   unfold merge_keys. *)
-  (*   induction ks2 using P.map_induction_bis; intros. *)
-  (*   - apply map_eq_Equal in H; subst; eauto. *)
-  (*   - invert H0. *)
-
-  (*   - rewrite fold_add; auto. *)
-  (*     rewrite merge_keys_notation; unfold add_key. *)
-  (*     cases (ks1 $k++ ks2 $? x); case (x ==n k_id); intros; subst; clean_map_lookups. *)
-  (*     + cases (k2 ==kk k0); subst. *)
-  (*       * eapply (merge_keys_came_from_somewhere1) in Heq; auto. rewrite Heq in H0; invert H0. rewrite canonical_key_refl. eapply merge_keys_adds_ks1; eauto. *)
-  (*       * eapply (merge_keys_came_from_somewhere1) in Heq; auto. rewrite Heq in H0; invert H0. rewrite canonical_key_sym. clean_map_lookups; trivial. *)
-  (*     + cases (e ==kk k0); subst; clean_map_lookups; eauto. *)
-  (*     + eapply merge_keys_no_disappear_keys in Heq; invert Heq; contra_map_lookup. *)
-  (*     + eapply IHks2; eauto. *)
-  (* Qed. *)
 
   (* Lemma add_key_results : *)
   (*   forall k v ks ks', *)
@@ -1601,296 +931,6 @@ Section KeyMergeTheorems.
   (*   cases (v ==kk k0); auto. *)
   (*   intuition eauto. *)
   (* Qed. *)
-
-  (* Lemma keys_compatible_reflexive : *)
-  (*   forall k, *)
-  (*     keys_compatible k k = true. *)
-  (* Proof. *)
-  (*   unfold keys_compatible; intros. *)
-  (*   cases (keyId k ==n keyId k); eauto. *)
-  (*   cases (keyUsage k ==ku keyUsage k); eauto. *)
-  (*   unfold key_type_same; cases (keyType k); eauto. *)
-  (* Qed. *)
-
-  (* Lemma keys_compatible_symmetric : *)
-  (*   forall k1 k2, *)
-  (*     keys_compatible k1 k2 = keys_compatible k2 k1. *)
-  (* Proof. *)
-  (*   unfold keys_compatible; intros. *)
-  (*   cases (keyId k1 ==n keyId k2). *)
-  (*   cases (keyUsage k1 ==ku keyUsage k2). *)
-  (*   cases (key_type_same (keyType k1) (keyType k2)). *)
-  (*   - rewrite e; rewrite e0; cases (keyId k2 ==n keyId k2); cases (keyUsage k2 ==ku keyUsage k2); try contradiction. *)
-  (*     unfold key_type_same in *; cases (keyType k1); cases (keyType k2); auto. *)
-  (*   - rewrite e; rewrite e0; cases (keyId k2 ==n keyId k2); cases (keyUsage k2 ==ku keyUsage k2); try contradiction. *)
-  (*     unfold key_type_same in *; cases (keyType k1); cases (keyType k2); auto. *)
-  (*   - rewrite e; cases (keyId k2 ==n keyId k2); auto. *)
-  (*     cases (keyUsage k2 ==ku keyUsage k1); auto. *)
-  (*     unfold key_type_same in *; cases (keyType k1); cases (keyType k2); auto. *)
-  (*   - cases (keyId k2 ==n keyId k1); cases (keyUsage k2 ==ku keyUsage k1); try contradiction; auto. *)
-  (*     symmetry in e; contradiction. *)
-  (* Qed. *)
-
-  (* Lemma merge_keys_ok : *)
-  (*   forall ks2 k_id k1 k2 ks ks1, *)
-  (*       ks1 $? k_id = Some k1 *)
-  (*     -> ks2 $? k_id = Some k2 *)
-  (*     -> ks = ks1 $k++ ks2 *)
-  (*     -> ( ks $? k_id = Some k1 /\ k1 = k2) *)
-  (*     \/ ( ks $? k_id = Some (canonical_key k1 k2)). *)
-  (* Proof. *)
-  (*   unfold merge_keys. *)
-  (*   induction ks2 using P.map_induction_bis; intros. *)
-
-  (*   - apply map_eq_Equal in H; subst; eauto. *)
-  (*   - invert H0. *)
-
-  (*   - subst. progress_fold_add1; clean_map_lookups; eauto. *)
-  (*     rewrite merge_keys_notation. *)
-  (*     case (x ==n k_id); intros; subst; clean_map_lookups. *)
-  (*     + remember (ks1 $k++ ks2) as ks. *)
-  (*       specialize (merge_keys_adds_ks1 _ _ _ H0 H Heqks). intros; subst. *)
-  (*       cases (k2 ==kk k1). *)
-  (*       * unfold add_key; subst. rewrite H1. *)
-  (*         rewrite canonical_key_refl; simpl. *)
-  (*         cases (k1 ==kk k1); try contradiction; eauto. *)
-
-  (*       * unfold add_key; rewrite H1; simpl. cases (k2 ==kk k1); try contradiction. *)
-  (*         rewrite canonical_key_sym. *)
-  (*         assert (k1 <> k2) by auto. *)
-
-  (*         clean_map_lookups; intuition idtac. *)
-
-  (*     + unfold add_key. *)
-  (*       cases (ks1 $k++ ks2 $? x); eauto. *)
-  (*       * cases (e ==kk k); clean_map_lookups; eauto. *)
-  (*       * clean_map_lookups; eauto. *)
-  (* Qed. *)
-
-  (* Lemma merge_keys_refl : *)
-  (*   forall ks, *)
-  (*     ks $k++ ks = ks. *)
-  (* Proof. *)
-  (*   intros; apply map_eq_Equal; unfold Equal; subst; intros. *)
-  (*   cases (ks $? y). *)
-  (*   - remember (ks $k++ ks) as ksks. *)
-  (*     pose proof (merge_keys_ok _ _ _ Heq Heq Heqksks). *)
-  (*     rewrite canonical_key_refl in *. *)
-  (*     intuition idtac. *)
-  (*   - rewrite merge_keys_adds_no_new_keys; eauto. *)
-  (* Qed. *)
-
-  (* Lemma merge_keys_symmetric : *)
-  (*   forall ks1 ks2, *)
-  (*     ks1 $k++ ks2 = ks2 $k++ ks1. *)
-  (* Proof. *)
-  (*   intros. *)
-
-  (*   apply map_eq_Equal; unfold Equal; subst; intros. *)
-
-  (*   cases (ks1 $? y); cases (ks2 $? y). *)
-  (*   - remember (ks1 $k++ ks2) as ks12. remember (ks2 $k++ ks1) as ks21. *)
-  (*     pose proof (merge_keys_ok _ _ _ Heq Heq0 Heqks12). *)
-  (*     pose proof (merge_keys_ok _ _ _ Heq0 Heq Heqks21). *)
-
-  (*     (repeat match goal with *)
-  (*             | [ H : _ /\ _ |- _ ] => destruct H; subst *)
-  (*             | [ H : _ \/ _ |- _ ] => destruct H *)
-  (*             | [ |- context [canonical_key ?k ?k]] => rewrite canonical_key_refl *)
-  (*             | [ H : _ $k++ _ $? _ = Some _ |- _ ] => rewrite H *)
-  (*             | [ H : _ $? _ = Some _ |- _ ] => rewrite H *)
-  (*             end); *)
-  (*       eauto. *)
-  (*     rewrite canonical_key_sym; trivial. *)
-
-  (*   - erewrite (merge_keys_adds_ks1); eauto. *)
-  (*     erewrite (merge_keys_adds_ks2); eauto. *)
-  (*   - erewrite (merge_keys_adds_ks2); eauto. *)
-  (*     erewrite (merge_keys_adds_ks1); eauto. *)
-  (*   - rewrite merge_keys_adds_no_new_keys; eauto. *)
-  (*     rewrite merge_keys_adds_no_new_keys; eauto. *)
-  (* Qed. *)
-
-  (* Hint Extern 1 (keys_compatible _ _ = _) => eassumption || (rewrite keys_compatible_symmetric; eassumption). *)
-
-  (* Lemma merge_keys_inequal_addition_no_impact : *)
-  (*   forall ks1 ks2 k_id k_id' k, *)
-  (*     k_id <> k_id' *)
-  (*     -> ks1 $k++ (ks2 $+ (k_id,k)) $? k_id' = ks1 $k++ ks2 $? k_id'. *)
-  (* Proof. *)
-  (*   intros. *)
-  (*   cases (ks1 $k++ ks2 $? k_id'). *)
-  (*   - apply merge_keys_split in Heq. *)
-  (*     split_ors; split_ands; subst. *)
-  (*     + eapply merge_keys_adds_ks2 with (ks2:=ks2 $+ (k_id, k)); clean_map_lookups; eauto. *)
-  (*     + eapply merge_keys_adds_ks1 with (ks2:=ks2 $+ (k_id, k)); clean_map_lookups; eauto. *)
-  (*     + destruct H0 as [k1 H0]. destruct H0 as [k2 H0]. split_ands. *)
-  (*       remember (ks1 $k++ ks2) as ks. *)
-  (*       specialize (merge_keys_ok _ _ _ H0 H1 Heqks); intros; split_ors; split_ands; subst. *)
-  (*       * rewrite canonical_key_refl. *)
-  (*         eapply merge_keys_canonicalizes' with (ks2:=ks2 $+ (k_id, k)). eauto. clean_map_lookups; eauto. rewrite canonical_key_refl; trivial. *)
-  (*       * eapply merge_keys_canonicalizes' with (ks2:=ks2 $+ (k_id, k)). eauto. clean_map_lookups; eauto. trivial. *)
-  (*   - apply merge_keys_no_disappear_keys in Heq; split_ands. *)
-  (*     eapply merge_keys_adds_no_new_keys; auto. *)
-  (*     clean_map_lookups; auto. *)
-  (* Qed. *)
-
-  (* Lemma merge_keys_assoc : *)
-  (*   forall ks3 ks1 ks2 : keys, *)
-  (*     ks1 $k++ ks2 $k++ ks3 = ks1 $k++ (ks2 $k++ ks3). *)
-  (* Proof. *)
-  (*   induction ks3 using P.map_induction_bis; intros. *)
-
-  (*   - apply map_eq_Equal in H; subst; eauto. *)
-  (*   - rewrite !merge_keys_right_identity; trivial. *)
-  (*   - apply map_eq_Equal; unfold Equal; subst; intros. *)
-  (*     unfold merge_keys. *)
-  (*     progress_fold_add1; auto. progress_fold_add1; auto. *)
-  (*     rewrite merge_keys_notation with (ks1 := ks1). *)
-  (*     rewrite merge_keys_notation with (ks2 := ks3). *)
-  (*     unfold add_key at 1; unfold add_key at 2. *)
-
-  (*     (* clean up notation of induction hypothesis *)  *)
-  (*     specialize (IHks3 ks1 ks2); unfold merge_keys in IHks3. *)
-  (*     rewrite merge_keys_notation  with (ks1 := ks1) in IHks3. *)
-  (*     rewrite merge_keys_notation  with (ks1 := ks2) in IHks3. *)
-  (*     rewrite merge_keys_notation  with (ks2 := ks3) in IHks3. *)
-  (*     rewrite merge_keys_notation  with (ks2 := ks2 $k++ ks3) in IHks3. *)
-
-  (*     rewrite merge_keys_notation with (ks1 := ks2). *)
-
-  (*     Ltac rewrite123 := *)
-  (*       match goal with | [ H : _ $k++ _ $k++ _ $? _ = _ |- _ ] => rewrite H end. *)
-
-  (*     cases (ks1 $k++ ks2 $k++ ks3 $? x); *)
-  (*       intros; subst; clean_map_lookups. *)
-
-  (*     + cases (ks2 $k++ ks3 $? x). *)
-  (*       * assert (ks1 $k++ ks2 $k++ ks3 $? x = Some k) as S by auto. *)
-  (*         rewrite IHks3 in S; eapply merge_keys_split in S; auto. *)
-  (*         cases (e ==kk k); cases (e ==kk k0); subst. *)
-  (*         ** rewrite merge_keys_notation with (ks2:=ks2$k++ks3); rewrite IHks3; trivial. *)
-  (*         ** rewrite merge_keys_notation with (ks2:=ks2 $k++ ks3 $+ (x, canonical_key k k0)). *)
-  (*            split_ors; split_ands; subst. *)
-  (*            *** rewrite Heq0 in H1; invert H1. contradiction. *)
-  (*            *** contra_map_lookup. *)
-  (*            *** destruct H0 as [k1 H0]. destruct H0 as [k2]. split_ands. rewrite Heq0 in H1; invert H1. symmetry. *)
-  (*                rewrite <- canonical_key_assoc. rewrite canonical_key_refl. *)
-  (*                cases (x ==n y); subst. *)
-  (*                  rewrite Heq. eapply merge_keys_canonicalizes'. eassumption. clean_map_lookups. reflexivity. rewrite canonical_key_assoc, canonical_key_refl; trivial. *)
-  (*                  rewrite IHks3. eapply merge_keys_inequal_addition_no_impact; assumption. *)
-  (*         ** rewrite merge_keys_notation with (ks2:=ks2$k++ks3). rewrite <- IHks3. *)
-  (*            split_ors; split_ands; subst. *)
-  (*            *** rewrite Heq0 in H1; invert H1. contradiction. *)
-  (*            *** contra_map_lookup. *)
-  (*            *** destruct H0 as [k1 H0]. destruct H0 as [k2]. split_ands. rewrite Heq0 in H1; invert H1. *)
-  (*                cases (x ==n y); subst. *)
-  (*                  rewrite canonical_key_sym, <- canonical_key_assoc, canonical_key_refl. clean_map_lookups; rewrite Heq; trivial. *)
-  (*                  clean_map_lookups; trivial. *)
-  (*         ** rewrite merge_keys_notation with (ks2:=ks2 $k++ ks3 $+ (x, canonical_key e k0)). *)
-  (*            split_ors; split_ands; subst. *)
-  (*            *** rewrite Heq0 in H1; invert H1. symmetry. *)
-  (*                cases (x ==n y); subst; clean_map_lookups. *)
-  (*                  eapply merge_keys_adds_ks2. eauto. 2:reflexivity. clean_map_lookups; trivial. *)
-  (*                  rewrite IHks3. eapply merge_keys_inequal_addition_no_impact; assumption. *)
-  (*            *** contra_map_lookup. *)
-  (*            *** destruct H0 as [k1 H0]. destruct H0 as [k2]. split_ands. rewrite Heq0 in H1; invert H1. *)
-  (*                symmetry. *)
-  (*                cases (x ==n y); subst; clean_map_lookups. *)
-  (*                **** eapply merge_keys_canonicalizes'; clean_map_lookups; eauto. *)
-  (*                     rewrite canonical_key_assoc, canonical_key_sym with (k1:=e), <- canonical_key_assoc; trivial. *)
-  (*                **** rewrite IHks3. eapply merge_keys_inequal_addition_no_impact; assumption. *)
-
-  (*       * cases (e ==kk k); subst. *)
-  (*         ** rewrite fold_add; auto. unfold add_key at 1. rewrite merge_keys_notation with (ks2:=ks2 $k++ ks3), <- IHks3. rewrite Heq. *)
-  (*            cases (k ==kk k); simpl; eauto. contradiction. *)
-  (*         ** rewrite fold_add; auto. unfold add_key at 1. rewrite merge_keys_notation with (ks2:=ks2 $k++ ks3), <- IHks3. rewrite Heq. *)
-  (*            cases (e ==kk k); simpl; eauto. contradiction. *)
-
-
-  (*     + assert (ks1 $k++ ks2 $k++ ks3 $? x = None) as HH by assumption; rewrite IHks3 in HH; eapply merge_keys_no_disappear_keys in HH; split_ands. *)
-  (*       rewrite H1. *)
-  (*       progress_fold_add1; auto. *)
-  (*       unfold add_key at 1. *)
-  (*       rewrite merge_keys_notation with (ks2:=ks2 $k++ ks3). rewrite <- IHks3. rewrite Heq; clean_map_lookups; trivial. *)
-  (* Qed. *)
-
-  (* Lemma findUserKeys_fold_fn_proper : *)
-  (*   forall {A}, *)
-  (*   Morphisms.Proper *)
-  (*     (Morphisms.respectful eq (Morphisms.respectful eq (Morphisms.respectful eq eq))) *)
-  (*     (fun (_ : NatMap.key) (u : user_data A) (ks : keys) => ks $k++ key_heap u). *)
-  (*   unfold Morphisms.Proper, Morphisms.respectful; intros; simpl; subst; trivial. *)
-  (* Qed. *)
-
-  (* Lemma findUserKeys_fold_fn_proper_Equal : *)
-  (*   forall {A}, *)
-  (*   Morphisms.Proper *)
-  (*     (Morphisms.respectful eq (Morphisms.respectful eq (Morphisms.respectful Equal Equal))) *)
-  (*     (fun (_ : NatMap.key) (u : user_data A) (ks : keys) => ks $k++ key_heap u). *)
-  (*   unfold Morphisms.Proper, Morphisms.respectful; intros. *)
-  (*   apply map_eq_Equal in H1; subst. *)
-  (*   unfold Equal; intros; trivial. *)
-  (* Qed. *)
-
-  (* Lemma findUserKeys_transpose : *)
-  (*   forall {A}, *)
-  (*     transpose_neqkey eq (fun (_ : NatMap.key) (u : user_data A) (ks : keys) => ks $k++ key_heap u). *)
-  (* Proof. *)
-  (*   unfold transpose_neqkey; intros. *)
-  (*   rewrite merge_keys_symmetric with (ks1 := a). *)
-  (*   rewrite merge_keys_symmetric with (ks1 := a $k++ key_heap e). *)
-  (*   rewrite merge_keys_assoc; trivial. *)
-  (* Qed. *)
-
-  (* Lemma findUserKeys_transpose_Equal : *)
-  (*   forall {A}, *)
-  (*     transpose_neqkey Equal (fun (_ : NatMap.key) (u : user_data A) (ks : keys) => ks $k++ key_heap u). *)
-  (* Proof. *)
-  (*   unfold transpose_neqkey; intros. *)
-  (*   unfold Equal; intros. *)
-  (*   rewrite merge_keys_symmetric with (ks1 := a). *)
-  (*   rewrite merge_keys_symmetric with (ks1 := a $k++ key_heap e). *)
-  (*   rewrite merge_keys_assoc; trivial. *)
-  (* Qed. *)
-
-  (* Hint Resolve findUserKeys_fold_fn_proper findUserKeys_fold_fn_proper_Equal findUserKeys_transpose findUserKeys_transpose_Equal. *)
-
-  (* TODO move to Maps.v *)
-  Lemma add_remove_eq :
-    forall {V} (m : NatMap.t V) k1 v1,
-      m $+ (k1, v1) $- k1 = m $- k1.
-  Proof.
-    intros. apply map_eq_Equal; unfold Equal; intros.
-    case (k1 ==n y); intros; subst.
-    - rewrite !remove_eq_o; auto.
-    - rewrite !remove_neq_o, add_neq_o; auto.
-  Qed.
-
-  Lemma add_remove_neq :
-    forall {V} (m : NatMap.t V) k1 v1 k2,
-        k1 <> k2
-      -> m $+ (k1, v1) $- k2 = m $- k2 $+ (k1, v1).
-  Proof.
-    intros. apply map_eq_Equal; unfold Equal; intros.
-    case (k2 ==n y); case (k1 ==n y); intros; subst.
-    - contradiction.
-    - rewrite add_neq_o by assumption; rewrite !remove_eq_o; trivial.
-    - rewrite remove_neq_o by assumption; rewrite !add_eq_o; trivial.
-    - rewrite remove_neq_o by assumption; rewrite !add_neq_o by assumption; rewrite remove_neq_o; auto.
-  Qed.
-
-  Lemma remove_not_in_idempotent :
-    forall {V} (m : NatMap.t V) k1,
-      m $? k1 = None
-      -> m $- k1 = m.
-  Proof.
-    intros.
-    eapply map_eq_Equal; unfold Equal; intros.
-    cases (y ==n k1); subst; eauto.
-    rewrite remove_eq_o by trivial; rewrite H; trivial.
-    rewrite remove_neq_o; auto.
-  Qed.
 
   (* Lemma find_user_keys_includes_user_keys: *)
   (*   forall {A} (us : honest_users A) u_id u_d, *)
@@ -1929,22 +969,22 @@ End KeyMergeTheorems.
 
 Definition sign_if_ok (c : cipher) (kt : key_type) (k : key_permission) : option cipher :=
   match (kt,k) with
-  | (SymKey,  MkKeyPerm _ _)      => Some c
-  | (AsymKey, MkKeyPerm _ true)   => Some c
-  | (AsymKey, MkKeyPerm _ false)  => None
+  | (SymKey,  (_, _))     => Some c
+  | (AsymKey, (_, true))  => Some c
+  | (AsymKey, (_, false)) => None
   end.
 
 Definition encryptMessage {t} (ks : keys) (k__sign k__enc : key_permission) (m : message t) (c_id : cipher_id) : option cipher :=
-  match (ks $? k__sign.(key_ref), ks $? k__enc.(key_ref)) with
+  match (ks $? fst k__sign, ks $? fst k__enc) with
   | (Some (MkCryptoKey _ Signing kt__sign), Some (MkCryptoKey _ Encryption kt__enc)) =>
-    sign_if_ok (SigEncCipher c_id k__sign.(key_ref) k__enc.(key_ref) m) kt__sign k__sign
+    sign_if_ok (SigEncCipher c_id (fst k__sign) (fst k__enc) m) kt__sign k__sign
   | _ => None
   end.
 
 Definition signMessage {t} (ks : keys) (k : key_permission) (m : message t) (c_id : cipher_id) : option cipher :=
-  match (ks $? k.(key_ref)) with
+  match ks $? fst k with
   | Some (MkCryptoKey _ Signing kt)     =>
-    sign_if_ok (SigCipher c_id k.(key_ref) m) kt k
+    sign_if_ok (SigCipher c_id (fst k) m) kt k
   | _ => None
   end.
 
@@ -2067,12 +1107,13 @@ Inductive step_user : forall A B C, rlabel -> data_step0 A B C -> data_step0 A B
                 (usrs', adv', cs, gks, ks, qmsgs, Return tt)
 
 (* Encryption / Decryption *)
-| StepEncrypt : forall {A B} {t} (usrs : honest_users A) (adv : user_data B) cs cs' gks ks qmsgs (msg : message t) k__sign k__enc k__signid k__encid c_id cipherMsg,
-      key_ref k__sign = k__signid
-    -> key_ref k__enc = k__encid
-    -> ks $? k__signid = Some k__sign
+| StepEncrypt : forall {A B} {t} (usrs : honest_users A) (adv : user_data B) cs cs' gks ks qmsgs (msg : message t)
+                  k__sign k__enc k__signid k__encid kp__sign kp__enc c_id cipherMsg,
+      k__sign = (k__signid, kp__sign)
+    -> k__enc  = (k__encid, kp__enc)
+    -> ks $? k__signid = Some (kp__sign)
     -> has_private_key gks k__sign = true
-    -> ks $? k__encid = Some k__enc
+    -> ks $? k__encid = Some (kp__enc)
     -> ~ In c_id cs
     -> encryptMessage gks k__sign k__enc msg c_id = Some cipherMsg
     -> cs' = cs $+ (c_id, cipherMsg)
@@ -2080,13 +1121,14 @@ Inductive step_user : forall A B C, rlabel -> data_step0 A B C -> data_step0 A B
                 (usrs, adv, cs , gks, ks, qmsgs, SignEncrypt k__sign k__enc msg)
                 (usrs, adv, cs', gks, ks, qmsgs, Return (SignedCiphertext c_id))
 
-| StepDecrypt : forall {A B} {t} (usrs : honest_users A) (adv : user_data B) cs gks ks ks' qmsgs (msg : message t) k__signid k__sign k__encid c_id newkeys kt b,
+| StepDecrypt : forall {A B} {t} (usrs : honest_users A) (adv : user_data B) cs gks ks ks' qmsgs (msg : message t)
+                  k__signid kp__sign k__encid c_id newkeys kt,
       cs $? c_id = Some (SigEncCipher c_id k__signid k__encid msg)
-    -> ( (gks $? k__encid = Some (MkCryptoKey k__encid Encryption SymKey)  /\ ks $? k__encid = Some (MkKeyPerm k__encid b))
-      \/ (gks $? k__encid = Some (MkCryptoKey k__encid Encryption AsymKey) /\ ks $? k__encid = Some (MkKeyPerm k__encid true))
+    -> ( (exists kp__enc, gks $? k__encid = Some (MkCryptoKey k__encid Encryption SymKey)  /\ ks $? k__encid = Some kp__enc)
+      \/ (gks $? k__encid = Some (MkCryptoKey k__encid Encryption AsymKey) /\ ks $? k__encid = Some true)
       )
     -> gks $? k__signid = Some (MkCryptoKey k__signid Signing kt)
-    -> ks $? k__signid = Some k__sign
+    -> ks $? k__signid = Some kp__sign
     -> findKeys msg = newkeys
     -> ks' = ks $k++ newkeys
     -> step_user Silent
@@ -2094,26 +1136,24 @@ Inductive step_user : forall A B C, rlabel -> data_step0 A B C -> data_step0 A B
                 (usrs, adv, cs, gks, ks', qmsgs, Return msg)
 
 (* Signing / Verification *)
-| StepSign : forall {A B} {t} (usrs : honest_users A) (adv : user_data B) cs cs' gks ks qmsgs (msg : message t) k k_id c_id cipherMsg,
-      key_ref k = k_id
-    -> ks $? k_id = Some k
-    -> has_private_key gks k = true
+| StepSign : forall {A B} {t} (usrs : honest_users A) (adv : user_data B) cs cs' gks ks qmsgs (msg : message t) kp k_id c_id cipherMsg,
+      ks $? k_id = Some kp
+    -> has_private_key gks (k_id,kp) = true
     -> ~(In c_id cs)
-    -> signMessage gks k msg c_id = Some cipherMsg
+    -> signMessage gks (k_id,kp) msg c_id = Some cipherMsg
     -> cs' = cs $+ (c_id, cipherMsg)
     -> step_user Silent
-                (usrs, adv, cs , gks, ks, qmsgs, Sign k msg)
+                (usrs, adv, cs , gks, ks, qmsgs, Sign (k_id,kp) msg)
                 (usrs, adv, cs', gks, ks, qmsgs, Return (Signature msg c_id))
 
-| StepVerify : forall {A B} {t} (usrs : honest_users A) (adv : user_data B) cs gks ks qmsgs (msg : message t) k_id k c_id,
-    key_ref k = k_id
+| StepVerify : forall {A B} {t} (usrs : honest_users A) (adv : user_data B) cs gks ks qmsgs (msg : message t) k_id kp c_id,
     (* k is in your key heap *)
-    -> ks $? (key_ref k) = Some k
+      ks $? k_id = Some kp
     (* return true or false whether k was used to sign the message *)
     -> cs $? c_id = Some (SigCipher c_id k_id msg)
     (* -> findKeys msg = newkeys *)
     -> step_user Silent
-                (usrs, adv, cs, gks, ks, qmsgs, (Verify k (Signature msg c_id)))
+                (usrs, adv, cs, gks, ks, qmsgs, (Verify (k_id,kp) (Signature msg c_id)))
                 (usrs, adv, cs, gks, ks, qmsgs, Return true)
                 (* (usrs, adv, cs, ks, qmsgs, Return (if (k_id ==n (keyId k)) then true else false)) *)
 .
@@ -2129,7 +1169,7 @@ Inductive step_user : forall A B C, rlabel -> data_step0 A B C -> data_step0 A B
 (*     -> k = AsymKey (MkCryptoKey kid usage) true *)
 (*     -> step_user (cs, ks, qmsgs, usrDat, GenerateAsymKey usage) *)
 (*                 (cs, ks $+ (kid, k), qmsgs, updateUserKeyHeap [k] usrDat, Return k) *)
-                
+
 (* | Barrier {result : Set} : user_cmd result. *)
 
 (* Lemma LStepRecv' : forall {B t} u_id (adv : adversaries B) globals globals' uks uks' (msg : message t) pat msgs newkeys, *)
